@prefix : <http://www.w3id.org/def/irrig#> .
@prefix owl: <http://www.w3.org/2002/07/owl#> .
@prefix rdf: <http://www.w3.org/1999/02/22-rdf-syntax-ns#> .
@prefix xml: <http://www.w3.org/XML/1998/namespace> .
@prefix xsd: <http://www.w3.org/2001/XMLSchema#> .
@prefix rdfs: <http://www.w3.org/2000/01/rdf-schema#> .
@base <http://www.w3id.org/def/irrig> .

<http://www.w3id.org/def/irrig> rdf:type owl:Ontology ;
                                 owl:versionIRI <http://www.w3id.org/def/irrig/201912> ;
                                 owl:imports <https://raw.githubusercontent.com/Irstea/caso/master/ontology/caso.owl> ;
                                 <http://purl.org/dc/elements/1.1/description> """IRRIG is an ontology specified for modeling data from a decision support system (DSS) experimented in UR1471 TSCF - Research Unit Technologies and Information Systems for Agrosystems, INRAE, center Clermont Ferrand. The DSS automatize the IRRINOV©, a manual irrigation method build by Arvalis and their partners. 
The website of TSCF: https://www6.ara.inrae.fr/tscf/"""@en ;
                                 <http://purl.org/dc/elements/1.1/publisher> <https://www6.clermont.inrae.fr/tscf> ;
                                 <http://purl.org/dc/elements/1.1/title> "Context Aware System Observation Ontology"@en ,
                                                                         "Irrigation ontology for experimentation in TSCF"@en ;
                                 <http://purl.org/dc/terms/contributor> <https://orcid.org/0000-0002-0421-452X> ,
                                                                        <https://orcid.org/0000-0002-7011-4535> ;
                                 <http://purl.org/dc/terms/creator> <https://orcid.org/0000-0002-3076-5499> ,
                                                                    <https://orcid.org/0000-0002-3517-0945> ,
                                                                    <https://orcid.org/0000-0003-3587-0367> ;
                                 <http://purl.org/dc/terms/license> <http://purl.org/NET/rdflicense/cc-by4.0> ;
                                 <http://purl.org/vocab/vann/preferredNamespacePrefix> "irrig" ;
                                 <http://purl.org/vocab/vann/preferredNamespaceUri> "http://www.w3id.org/def/irrig#"^^xsd:anyURI ;
                                 owl:versionInfo "1.2.0" .

#################################################################
#    Annotation properties
#################################################################

###  http://www.w3.org/2004/02/skos/core#definition
<http://www.w3.org/2004/02/skos/core#definition> rdf:type owl:AnnotationProperty .


###  http://www.w3.org/2004/02/skos/core#example
<http://www.w3.org/2004/02/skos/core#example> rdf:type owl:AnnotationProperty .


###  http://www.w3.org/2004/02/skos/core#note
<http://www.w3.org/2004/02/skos/core#note> rdf:type owl:AnnotationProperty .


#################################################################
#    Object Properties
#################################################################

###  http://www.w3.org/ns/prov#wasDerivedFrom
<http://www.w3.org/ns/prov#wasDerivedFrom> rdf:type owl:ObjectProperty ;
                                           rdfs:subPropertyOf <http://www.w3.org/ns/prov#wasInfluencedBy> ;
                                           rdfs:comment "A derivation is a transformation of an entity into another, an update of an entity resulting in a new one, or the construction of a new entity based on a pre-existing entity."@en ;
                                           rdfs:label "wasDerivedFrom" .


#################################################################
#    Data properties
#################################################################

###  https://w3id.org/saref#hasManufacturer
<https://w3id.org/saref#hasManufacturer> rdf:type owl:DatatypeProperty ;
                                         rdfs:range xsd:string ;
                                         rdfs:comment "A relationship identifying the manufacturer of an entity (e.g., device)" ;
                                         rdfs:label "has manufacturer" .


###  https://w3id.org/saref#hasModel
<https://w3id.org/saref#hasModel> rdf:type owl:DatatypeProperty ;
                                  rdfs:range xsd:string ;
                                  rdfs:comment "A relationship identifying the model of an entity (e.g., device)" ;
                                  rdfs:label "has model" .


###  https://w3id.org/saref#hasName
<https://w3id.org/saref#hasName> rdf:type owl:DatatypeProperty ;
                                 rdfs:range xsd:string ;
                                 rdfs:comment "A relationship providing the name of an entity (e.g., device)" ;
                                 rdfs:label "has name" .


#################################################################
#    Classes
#################################################################

###  http://www.w3id.org/def/caso#Property
<http://www.w3id.org/def/caso#Property> owl:equivalentClass [ owl:intersectionOf ( <http://www.w3id.org/def/caso#Observation>
                                                                                   [ rdf:type owl:Restriction ;
                                                                                     owl:onProperty <http://www.w3.org/ns/sosa/observedProperty> ;
                                                                                     owl:hasValue :observableProperty_delayDuration
                                                                                   ]
                                                                                 ) ;
                                                              rdf:type owl:Class
                                                            ] .


###  http://www.w3id.org/def/irrig#AmountProperty
:AmountProperty rdf:type owl:Class ;
                rdfs:subClassOf <http://www.w3.org/ns/ssn/Property> ;
                rdfs:comment "AmountProperty - Amount or quantity aspect of an entity. The amount aspect of an entity is intrinsic and cannot exist without the entity. The value of the amount should be expressed by a qualitative value such as a state or by a quantitative value."@en ;
                rdfs:label "Amount Property" ;
                <http://www.w3.org/2004/02/skos/core#example> "RainQuantity is an AmountProperty representing the amount of rain."@en .


###  http://www.w3id.org/def/irrig#CropGrowthDeduction
:CropGrowthDeduction rdf:type owl:Class ;
                     owl:equivalentClass [ owl:intersectionOf ( <http://www.w3id.org/def/caso#Deduction>
                                                                [ rdf:type owl:Restriction ;
                                                                  owl:onProperty <http://www.w3.org/ns/sosa/hasFeatureOfInterest> ;
                                                                  owl:hasValue :featureOfInterest_crop
                                                                ]
                                                                [ rdf:type owl:Restriction ;
                                                                  owl:onProperty <http://www.w3.org/ns/sosa/observedProperty> ;
                                                                  owl:hasValue :observableProperty_crop_growth
                                                                ]
                                                              ) ;
                                           rdf:type owl:Class
                                         ] ;
                     rdfs:subClassOf <http://www.w3id.org/def/caso#Deduction> ;
                     rdfs:comment "CropGrowthDeduction - A defined class that represents the act of carrying out a procedure to estimate the state of the growth property for the crop entity. The growth property is represented by the individual irrig:observableProperty_crop_growth. The crop entity is represented by the individual irrig:featureOfInterest_crop. Two necessary and sufficient conditions are defined: (1) All instances of this class are linked to the individual irrig:observableProperty_crop_growth via the sosa:observedProperty object property; (2) All instance of this class are linked to the individual irrig:featureOfInterest_crop via the sosa:hasFeatureOfInterest object property. Additionally, each instance of this class is linked to an instance of the class irrig:CropGrowthState by the caso:hasResultState object property, is linked to an instance of the class irrig:CropGrowthObservation by the prov:wasInformedBy object property, and is linked to a sensor to describe the agent that made the deduction."@en ;
                     rdfs:label "Crop Growth Deduction"@en ;
                     <http://www.w3.org/2004/02/skos/core#example> "A CropGrowthDeduction is made by an inference engine based on human observation."@en .


###  http://www.w3id.org/def/irrig#CropGrowthObservation
:CropGrowthObservation rdf:type owl:Class ;
                       owl:equivalentClass [ owl:intersectionOf ( <http://www.w3id.org/def/caso#Observation>
                                                                  [ rdf:type owl:Restriction ;
                                                                    owl:onProperty <http://www.w3.org/ns/sosa/hasFeatureOfInterest> ;
                                                                    owl:hasValue :featureOfInterest_crop
                                                                  ]
                                                                  [ rdf:type owl:Restriction ;
                                                                    owl:onProperty <http://www.w3.org/ns/sosa/observedProperty> ;
                                                                    owl:hasValue :observableProperty_crop_growth
                                                                  ]
                                                                ) ;
                                             rdf:type owl:Class
                                           ] ;
                       rdfs:subClassOf <http://www.w3id.org/def/caso#Observation> ;
                       rdfs:comment "CropGrowthObservation - A defined class that represents the act of carrying out a procedure (observation) to estimate the value of the growth property for the crop entity. The growth property is represented by the individual irrig:observableProperty_crop_growth. The crop entity is represented by the individual irrig:featureOfInterest_crop. Two necessary and sufficient conditions are defined: (1) All instances of this class are linked to the individual irrig:observableProperty_crop_growth} via the sosa:observedProperty object property; (2) All instance of this class are linked to the individual irrig:featureOfInterest_crop} via the sosa:hasFeatureOfInterest object property. Additionally, each instance of this class is linked to a sensor to describe the agent that made the observation."@en ;
                       rdfs:label "Crop Growth Observation"@en ;
                       <http://www.w3.org/2004/02/skos/core#example> "A CropGrowthObservation that made by a famer called John Doe."@en .


###  http://www.w3id.org/def/irrig#CropGrowthState
:CropGrowthState rdf:type owl:Class ;
                 rdfs:subClassOf <http://www.w3id.org/def/caso#State> ;
                 rdfs:comment "CropGrowthState - A qualitative value of the crop growth property, which changes over time, summarising a set of information about that property. To evaluate the state of the property, some boundaries need to be defined."@en ;
                 rdfs:label "Crop Growth State"@en ;
                 <http://www.w3.org/2004/02/skos/core#example> "A state V2 is linked to an individual of the CropGrowth property dedicated to maize crop. The state V2 is reached when two leaves have fully emerged with collars visible in a maize plant."@en .


###  http://www.w3id.org/def/irrig#CropWaterNeedDeduction
:CropWaterNeedDeduction rdf:type owl:Class ;
                        owl:equivalentClass [ owl:intersectionOf ( <http://www.w3id.org/def/caso#Deduction>
                                                                   [ rdf:type owl:Restriction ;
                                                                     owl:onProperty <http://www.w3.org/ns/sosa/hasFeatureOfInterest> ;
                                                                     owl:hasValue :featureOfInterest_crop
                                                                   ]
                                                                   [ rdf:type owl:Restriction ;
                                                                     owl:onProperty <http://www.w3.org/ns/sosa/observedProperty> ;
                                                                     owl:hasValue :observableProperty_crop_waterNeed
                                                                   ]
                                                                 ) ;
                                              rdf:type owl:Class
                                            ] ;
                        rdfs:subClassOf <http://www.w3id.org/def/caso#Deduction> ;
                        rdfs:comment "CropWaterNeedDeduction - a defined class represents act of carrying out an (Observation) Procedure to estimate a State of the irrig:ObservableProperty_crop_waterNeed of the irrig:FeatureOfInterest_crop. The Observation may be performed by an inference engine. Links to a State to describe what the result is. Links to a TemporalEntity to indicate when the result is valid and for how many time."@en ;
                        rdfs:label "Crop Water Need Deduction"@en ;
                        <http://www.w3.org/2004/02/skos/core#example> "A CropWaterNeedDeduction that made by an inference engine based on the state of the other properties such as RainIntensity property."@en .


###  http://www.w3id.org/def/irrig#CropWaterNeedState
:CropWaterNeedState rdf:type owl:Class ;
                    rdfs:subClassOf <http://www.w3id.org/def/caso#State> ;
                    rdfs:comment "CropWaterNeedState - A qualitative value of the crop water need property, which changes over time, summarizing a set of information about that property. To evaluate the state of the property, some boundaries need to be defined."@en ;
                    rdfs:label "Crop Water Need State"@en ;
                    <http://www.w3.org/2004/02/skos/core#example> "The state No of the crop water need Property represents the fact that the crop does not need water."@en .


###  http://www.w3id.org/def/irrig#DelayDurationObservation
:DelayDurationObservation rdf:type owl:Class ;
                          owl:equivalentClass [ owl:intersectionOf ( <http://www.w3id.org/def/caso#Observation>
                                                                     [ rdf:type owl:Restriction ;
                                                                       owl:onProperty <http://www.w3.org/ns/sosa/hasFeatureOfInterest> ;
                                                                       owl:hasValue :featureOfInterest_delay
                                                                     ]
                                                                     [ rdf:type owl:Restriction ;
                                                                       owl:onProperty <http://www.w3.org/ns/sosa/observedProperty> ;
                                                                       owl:hasValue :observableProperty_delayDuration
                                                                     ]
                                                                   ) ;
                                                rdf:type owl:Class
                                              ] ;
                          rdfs:subClassOf <http://www.w3id.org/def/caso#Observation> ;
                          rdfs:comment "DelayDurationObservation - a defined class that represents act of carrying out a procedure (observation) to calculate the number of delay days of the duration property for the delay entity. Delay days are the number of days that the system postpones the schedule. The duration property is represented by the individual irrig:observableProperty_delayDuration. The delay entity is represented by the individual irrig:featureOfInterest_delay. Two necessary and sufficient conditions are defined: (1) All instances of this class are linked to the individual irrig:observableProperty_delayDuration via the sosa:observedProperty object property; (2) All instance of this class are linked to the individual irrig:featureOfInterest_delay} via the sosa:hasFeatureOfInterest object property. Additionally, each instance of this class is linked to a sensor to describe the agent that made the observation."@en ;
                          rdfs:label "Delay Duration Observation" ;
                          <http://www.w3.org/2004/02/skos/core#example> "A delay duration to postpone the irrigation schedule is two days."@en .


###  http://www.w3id.org/def/irrig#GrowthProperty
:GrowthProperty rdf:type owl:Class ;
                rdfs:subClassOf <http://www.w3.org/ns/ssn/Property> ;
                rdfs:comment "GrowthProperty - Growth aspect of an entity representing the physical development or the increasing of amount, number, or size of the entity. The growth aspect of an entity is intrinsic and cannot exist without the entity. The growth quality should be expressed by a qualitative value such as a state or by a quantitative value."@en ;
                rdfs:label "Growth Property"@en ;
                <http://www.w3.org/2004/02/skos/core#example> "CropGrowth is a growth property representing the development of a crop."@en .


###  http://www.w3id.org/def/irrig#IntensityProperty
:IntensityProperty rdf:type owl:Class ;
                   rdfs:subClassOf <http://www.w3.org/ns/ssn/Property> ;
                   rdfs:comment "IntensityProperty - Intensity aspect of an entity, that is,  the strong effect or the level of power per unit area of the entity. The intensity aspect of an entity is intrinsic and cannot exist without the entity. The intensity quality should be expressed by a qualitative value such as a state or by a quantitative value."@en ;
                   rdfs:label "Intensity Property"@en ;
                   <http://www.w3.org/2004/02/skos/core#example> "RainIntensity is an intensity representing the strength of rain."@en .


###  http://www.w3id.org/def/irrig#IrrigationActuation
:IrrigationActuation rdf:type owl:Class ;
                     owl:equivalentClass [ rdf:type owl:Class ;
                                           owl:unionOf ( [ owl:intersectionOf ( <http://www.w3id.org/def/caso#Actuation>
                                                                                [ owl:intersectionOf ( [ rdf:type owl:Restriction ;
                                                                                                         owl:onProperty <http://www.w3.org/ns/sosa/actsOnProperty> ;
                                                                                                         owl:hasValue :observableProperty_soil60cmDepth_moisture
                                                                                                       ]
                                                                                                       [ rdf:type owl:Restriction ;
                                                                                                         owl:onProperty <http://www.w3.org/ns/sosa/hasFeatureOfInterest> ;
                                                                                                         owl:hasValue :featureOfInterest_soil60cmDepth
                                                                                                       ]
                                                                                                     ) ;
                                                                                  rdf:type owl:Class
                                                                                ]
                                                                              ) ;
                                                           rdf:type owl:Class
                                                         ]
                                                         [ owl:intersectionOf ( [ rdf:type owl:Restriction ;
                                                                                  owl:onProperty <http://www.w3.org/ns/sosa/actsOnProperty> ;
                                                                                  owl:hasValue :observableProperty_soil30cmDepth_moisture
                                                                                ]
                                                                                [ rdf:type owl:Restriction ;
                                                                                  owl:onProperty <http://www.w3.org/ns/sosa/hasFeatureOfInterest> ;
                                                                                  owl:hasValue :featureOfInterest_soil30cmDepth
                                                                                ]
                                                                              ) ;
                                                           rdf:type owl:Class
                                                         ]
                                                       )
                                         ] ;
                     rdfs:subClassOf <http://www.w3id.org/def/caso#Actuation> ;
                     rdfs:comment "IrrigationActuation - Act of carrying out an Irrigation (Actuation) Procedure to change the State of a Moisture ActuatableProperty of a Soil FeatureOfInterest using a watering Actuator. This act is performed during the context exploitation phase of a context aware system. Links to an Actuator to describe what made the Actuation and how; links to an ActuatableProperty to describe the target that the Actuation change; links to a FeatureOfInterest to detail what that property was associated with. When the act is performed based on a Deduction, it should be linked to this Deduction by the wasInfluencedBy property. Links to the Function that is triggered by the Actuation."@en ;
                     rdfs:label "Irrigation actuation"@en ;
                     <http://www.w3.org/2004/02/skos/core#example> "An IrrigationActuation is made by Watering Valve Actuator, links to Soil30cmDepth FeatureOfInterest and its Soil30cmDepthMoisture ActuatableProperty."@en .


###  http://www.w3id.org/def/irrig#MoistureProperty
:MoistureProperty rdf:type owl:Class ;
                  rdfs:subClassOf <http://www.w3.org/ns/ssn/Property> ;
                  rdfs:comment "MoistureProperty - Moisture aspect of an entity representing the amount of water available inside the entity. The moisture aspect of the entity is intrinsic to and cannot exist without the entity. The moisture quality should be expressed by a qualitative value such as States or by a quantitative value."@en ;
                  rdfs:label "Moisture Property"@en ;
                  <http://www.w3.org/2004/02/skos/core#example> "RootZoneMoistureLevel is a MoistureProperty representing the amount of water available around the soil’s root zone area of a plant."@en .


###  http://www.w3id.org/def/irrig#RainDailyTotalQuantityObservation
:RainDailyTotalQuantityObservation rdf:type owl:Class ;
                                   owl:equivalentClass [ owl:intersectionOf ( <http://www.w3id.org/def/caso#Observation>
                                                                              [ rdf:type owl:Restriction ;
                                                                                owl:onProperty <http://www.w3.org/ns/sosa/hasFeatureOfInterest> ;
                                                                                owl:hasValue :featureOfInterest_rain
                                                                              ]
                                                                              [ rdf:type owl:Restriction ;
                                                                                owl:onProperty <http://www.w3.org/ns/sosa/observedProperty> ;
                                                                                owl:hasValue :observableProperty_rain_dailyTotalQuantity
                                                                              ]
                                                                            ) ;
                                                         rdf:type owl:Class
                                                       ] ;
                                   rdfs:subClassOf <http://www.w3id.org/def/caso#Observation> ;
                                   rdfs:comment "RainQuantityObservation - a defined class that represents act of carrying out an (Observation) Procedure to estimate or calculate a value of the irrig:ObservableProperty_rain_dailyTotalQuantity of the irrig:FeatureOfInterest_rain. This act can be performed during the context acquisition or context processing phases of a context aware system. Links to a Sensor to describe what made the Observation and how; links to the irrig:ObservableProperty_rain_dailyTotalQuantity to describe what the result is an estimate of, and to the irrig:FeatureOfInterest_rain. When the act is made during the context processing phase the entry values of the procedure should be linked to the Observation by the wasDerivedFrom property."@en ;
                                   rdfs:label "Rain Daily Total Quantity Observation"@en ;
                                   <http://www.w3.org/2004/02/skos/core#example> "A RainDailyTotalQuantityObservation is based on observations made by an aggregator."@en .


###  http://www.w3id.org/def/irrig#RainIntensityBoundary
:RainIntensityBoundary rdf:type owl:Class ;
                       rdfs:subClassOf <http://www.w3id.org/def/caso#Boundary> ;
                       rdfs:comment "RainIntensityBoundary - Limit of a state of the rain intensity property. The value of the limit is quantitative. The irrig:boundaryValue data property is used to store this value."@en ;
                       rdfs:label "Rain Intensity Boundary"@en ;
                       <http://www.w3.org/2004/02/skos/core#example> "10 mm is the value of the low boundary that distinguishes the light state from the moderate state of the rain intensity property."@en .


###  http://www.w3id.org/def/irrig#RainIntensityDeduction
:RainIntensityDeduction rdf:type owl:Class ;
                        owl:equivalentClass [ owl:intersectionOf ( <http://www.w3id.org/def/caso#Deduction>
                                                                   [ rdf:type owl:Restriction ;
                                                                     owl:onProperty <http://www.w3.org/ns/sosa/hasFeatureOfInterest> ;
                                                                     owl:hasValue :featureOfInterest_rain
                                                                   ]
                                                                   [ rdf:type owl:Restriction ;
                                                                     owl:onProperty <http://www.w3.org/ns/sosa/observedProperty> ;
                                                                     owl:hasValue :observableProperty_rain_intensity
                                                                   ]
                                                                 ) ;
                                              rdf:type owl:Class
                                            ] ;
                        rdfs:subClassOf <http://www.w3id.org/def/caso#Deduction> ;
                        rdfs:comment "RainIntensityDeduction - a defined class that represents act of carrying out a procedure to estimate the state of the intensity property for the rain entity. The intensity property is represented by the individual irrig:observableProperty_rain_intensity. The rain entity is represented by the individual irrig:featureOfInterest_rain. Two necessary and sufficient conditions are defined: (1) All instances of this class are linked to the individual irrig:observableProperty_rain_intensity via the sosa:observedProperty object property; (2) All instances of this class are linked to the individual irrig:featureOfInterest_rain via the sosa:hasFeatureOfInterest object property. Additionally, each instance of this class is linked to an instance of the class irrig:RainIntensityState by the caso:hasResultState object property; is linked to an instance of the class irrig:RainDailyTotalQuantityObservation by the prov:wasInformedBy object property; and is linked to a sensor to describe the agent that made the deduction."@en ;
                        rdfs:label "Rain Intensity Deduction"@en ;
                        <http://www.w3.org/2004/02/skos/core#example> "A RainIntensityDeduction that made by an inference engine based on observations made by an aggregator."@en .


###  http://www.w3id.org/def/irrig#RainIntensityState
:RainIntensityState rdf:type owl:Class ;
                    owl:equivalentClass [ owl:intersectionOf ( <http://www.w3id.org/def/caso#State>
                                                               [ rdf:type owl:Class ;
                                                                 owl:unionOf ( [ rdf:type owl:Restriction ;
                                                                                 owl:onProperty <http://www.w3id.org/def/caso#hasClosedLowerBoundary> ;
                                                                                 owl:someValuesFrom :RainIntensityBoundary
                                                                               ]
                                                                               [ rdf:type owl:Restriction ;
                                                                                 owl:onProperty <http://www.w3id.org/def/caso#hasOpenLowerBoundary> ;
                                                                                 owl:someValuesFrom :RainIntensityBoundary
                                                                               ]
                                                                             )
                                                               ]
                                                               [ rdf:type owl:Class ;
                                                                 owl:unionOf ( [ rdf:type owl:Restriction ;
                                                                                 owl:onProperty <http://www.w3id.org/def/caso#hasClosedUpperBoundary> ;
                                                                                 owl:someValuesFrom :RainIntensityBoundary
                                                                               ]
                                                                               [ rdf:type owl:Restriction ;
                                                                                 owl:onProperty <http://www.w3id.org/def/caso#hasOpenUpperBoundary> ;
                                                                                 owl:someValuesFrom :RainIntensityBoundary
                                                                               ]
                                                                             )
                                                               ]
                                                             ) ;
                                          rdf:type owl:Class
                                        ] ;
                    rdfs:subClassOf <http://www.w3id.org/def/caso#State> ;
                    rdfs:comment "RainIntensityState - Qualitative value of the rain intensity property, which changes over time, summarizing a set of information about that property. To evaluate the state of the property, some boundaries need to be defined."@en ;
                    rdfs:label "Rain Intensity State"@en ;
                    <http://www.w3.org/2004/02/skos/core#example> "The state Light of the RainIntensity property represents the fact that the rain has no impact on irrigation decisions."@en .


###  http://www.w3id.org/def/irrig#RainQuantityObservation
:RainQuantityObservation rdf:type owl:Class ;
                         owl:equivalentClass [ owl:intersectionOf ( <http://www.w3id.org/def/caso#Observation>
                                                                    [ rdf:type owl:Restriction ;
                                                                      owl:onProperty <http://www.w3.org/ns/sosa/hasFeatureOfInterest> ;
                                                                      owl:hasValue :featureOfInterest_rain
                                                                    ]
                                                                    [ rdf:type owl:Restriction ;
                                                                      owl:onProperty <http://www.w3.org/ns/sosa/observedProperty> ;
                                                                      owl:hasValue :observableProperty_rain_quantity
                                                                    ]
                                                                  ) ;
                                               rdf:type owl:Class
                                             ] ;
                         rdfs:subClassOf <http://www.w3id.org/def/caso#Observation> ;
                         rdfs:comment "RainQuantityObservation - A defined class that represents the act of carrying out a procedure (observation) to estimate the value of the quantity property for the rain entity. The quantity property is represented by the individual irrig:observableProperty_rain_quantity. The rain entity is represented by the individual irrig:featureOfInterest_rain. Two necessary and sufficient conditions are defined: (1) All instances of this class are linked to the individual irrig:observableProperty_rain_quantity via the sosa:observedProperty object property; (2) All instances of this class are linked to the individual irrig:featureOfInterest_rain via the sosa:hasFeatureOfInterest object property. Additionally, each instance of this class is linked to a sensor to describe the agent that made the observation."@en ;
                         rdfs:label "Rain Quantity Observation"@en ;
                         <http://www.w3.org/2004/02/skos/core#example> "A RainQuantityObservation that made by a pluviometer."@en .


###  http://www.w3id.org/def/irrig#RootZoneDailyAverageMoistureObservation
:RootZoneDailyAverageMoistureObservation rdf:type owl:Class ;
                                         owl:equivalentClass [ owl:intersectionOf ( <http://www.w3id.org/def/caso#Observation>
                                                                                    [ rdf:type owl:Restriction ;
                                                                                      owl:onProperty <http://www.w3.org/ns/sosa/hasFeatureOfInterest> ;
                                                                                      owl:hasValue :featureOfInterest_rootZone
                                                                                    ]
                                                                                    [ rdf:type owl:Restriction ;
                                                                                      owl:onProperty <http://www.w3.org/ns/sosa/observedProperty> ;
                                                                                      owl:hasValue :observableProperty_rootZone_dailyAverageMoisture
                                                                                    ]
                                                                                  ) ;
                                                               rdf:type owl:Class
                                                             ] ;
                                         rdfs:subClassOf <http://www.w3id.org/def/caso#Observation> ;
                                         rdfs:comment "RootZoneDailyAverageMoistureObservation - A defined class that represents the act of carrying out a procedure (observation) to estimate the value of the daily average moisture property for the root zone entity. The daily moisture property is represented by the individual irrig:observableProperty_rootZone_dailyAverageMoisture. The root zone entity is represented by the individual irrig:featureOfInterest_rootZone. Two necessary and sufficient conditions are defined: (1) All instances of this class are linked to the individual irrig:observableProperty_rootZone_dailyAverageMoisture via the sosa:observedProperty object property; (2) All instances of this class are linked to the individual irrig:featureOfInterest_rootZone via the sosa:hasFeatureOfInterest object property. Additionally, each instance of this class is linked to a sensor to describe the agent that made the observation."@en ;
                                         rdfs:label "Root Zone Daily Moisture Observation"@en ;
                                         <http://www.w3.org/2004/02/skos/core#example> "A RootZoneDailyAverageMoistureObservation is computed by an aggregator."@en .


###  http://www.w3id.org/def/irrig#RootZoneMoistureLevelBoundary
:RootZoneMoistureLevelBoundary rdf:type owl:Class ;
                               rdfs:subClassOf <http://www.w3id.org/def/caso#Boundary> ;
                               rdfs:comment "RootZoneMoistureLevelBoundary - Limit of a state of the root zone moisture level property. The value of the limit is quantitative. To store this value, the irrig:boundaryValue data property is used."@en ;
                               rdfs:label "Root Zone Moisture Level Boundary"@en ;
                               <http://www.w3.org/2004/02/skos/core#example> "10 cbar is the value of the very high tension boundary that distinguishes the saturated state from the very high state of the RootZoneMoistureLevel property."@en .


###  http://www.w3id.org/def/irrig#RootZoneMoistureLevelDeduction
:RootZoneMoistureLevelDeduction rdf:type owl:Class ;
                                owl:equivalentClass [ owl:intersectionOf ( <http://www.w3id.org/def/caso#Deduction>
                                                                           [ rdf:type owl:Restriction ;
                                                                             owl:onProperty <http://www.w3.org/ns/sosa/hasFeatureOfInterest> ;
                                                                             owl:hasValue :featureOfInterest_rootZone
                                                                           ]
                                                                           [ rdf:type owl:Restriction ;
                                                                             owl:onProperty <http://www.w3.org/ns/sosa/observedProperty> ;
                                                                             owl:hasValue :observableProperty_rootZone_moistureLevel
                                                                           ]
                                                                         ) ;
                                                      rdf:type owl:Class
                                                    ] ;
                                rdfs:subClassOf <http://www.w3id.org/def/caso#Deduction> ;
                                rdfs:comment "RootZoneMoistureLevelDeduction - A defined class that represents the act of carrying out a procedure to estimate the state of the moisture level property for the root zone entity. The moisture level property is represented by the individual irrig:observableProperty_rootZone_moistureLevel. The root zone entity is represented by the individual irrig:featureOfInterest_rootZone. Two necessary and sufficient conditions are defined: (1) All instances of this class are linked to the individual irrig:observableProperty_rootZone_moistureLevel} via the sosa:observedProperty object property; (2) All instances of this class are linked to the individual irrig:featureOfInterest_rootZone via the sosa:hasFeatureOfInterest object property. Additionally, each instance of this class is linked to an instance of the class irrig:RootZoneMoistureLevelState by the caso:hasResultState object property; is linked to an instance of the class irrig:RootZoneDailyAverageMoistureObservation by the prov:wasInformedBy object property; and is linked to a sensor to describe the agent that made the deduction."@en ;
                                rdfs:label "Root Zone Moisture Level Deduction"@en ;
                                <http://www.w3.org/2004/02/skos/core#example> "A RootZoneMoistureLevelDeduction that made by an inference engine based on observations from an aggregator."@en .


###  http://www.w3id.org/def/irrig#RootZoneMoistureLevelState
:RootZoneMoistureLevelState rdf:type owl:Class ;
                            owl:equivalentClass [ owl:intersectionOf ( <http://www.w3id.org/def/caso#State>
                                                                       [ rdf:type owl:Class ;
                                                                         owl:unionOf ( [ rdf:type owl:Restriction ;
                                                                                         owl:onProperty <http://www.w3id.org/def/caso#hasClosedLowerBoundary> ;
                                                                                         owl:someValuesFrom :RootZoneMoistureLevelBoundary
                                                                                       ]
                                                                                       [ rdf:type owl:Restriction ;
                                                                                         owl:onProperty <http://www.w3id.org/def/caso#hasOpenLowerBoundary> ;
                                                                                         owl:someValuesFrom :RootZoneMoistureLevelBoundary
                                                                                       ]
                                                                                     )
                                                                       ]
                                                                       [ rdf:type owl:Class ;
                                                                         owl:unionOf ( [ rdf:type owl:Restriction ;
                                                                                         owl:onProperty <http://www.w3id.org/def/caso#hasClosedUpperBoundary> ;
                                                                                         owl:someValuesFrom :RootZoneMoistureLevelBoundary
                                                                                       ]
                                                                                       [ rdf:type owl:Restriction ;
                                                                                         owl:onProperty <http://www.w3id.org/def/caso#hasOpenUpperBoundary> ;
                                                                                         owl:someValuesFrom :RootZoneMoistureLevelBoundary
                                                                                       ]
                                                                                     )
                                                                       ]
                                                                     ) ;
                                                  rdf:type owl:Class
                                                ] ;
                            rdfs:subClassOf <http://www.w3id.org/def/caso#State> ;
                            rdfs:comment "RootZoneMoistureLevelState - Qualitative value of the root zone moisture level property, which changes over time, summarizing a set of information about that property. To evaluate the state of the property, some boundaries need to be defined."@en ;
                            rdfs:label "Root Zone Moisture Level State"@en ;
                            <http://www.w3.org/2004/02/skos/core#example> "The saturated state of the RootZoneMoistureLevel Property represents a fact that the moisture in the root zone is saturated with water."@en .


###  http://www.w3id.org/def/irrig#SleepingDurationObservation
:SleepingDurationObservation rdf:type owl:Class ;
                             owl:equivalentClass [ owl:intersectionOf ( <http://www.w3id.org/def/caso#Observation>
                                                                        [ rdf:type owl:Restriction ;
                                                                          owl:onProperty <http://www.w3.org/ns/sosa/hasFeatureOfInterest> ;
                                                                          owl:hasValue :featureOfInterest_sleeping
                                                                        ]
                                                                        [ rdf:type owl:Restriction ;
                                                                          owl:onProperty <http://www.w3.org/ns/sosa/observedProperty> ;
                                                                          owl:hasValue :observableProperty_sleepingDuration
                                                                        ]
                                                                      ) ;
                                                   rdf:type owl:Class
                                                 ] ;
                             rdfs:subClassOf <http://www.w3id.org/def/caso#Observation> ;
                             rdfs:comment "SleepingDurationObservation - A defined class that represents the act of carrying out a procedure (observation) to calculate the number of sleeping days of the duration property for the sleeping entity. Sleeping days are the number of days that the system needs to wait until the next turn of doing an action. The duration property is represented by the individual irrig:observableProperty_sleepingDuration. The sleeping entity is represented by the individual irrig:featureOfInterest_sleeping. Two necessary and sufficient conditions are defined: (1) All instances of this class are linked to the individual irrig:observableProperty_sleepingDuration via the sosa:observedProperty object property; (2) All instances of this class are linked to the individual irrig:featureOfInterest_sleeping via the sosa:hasFeatureOfInterest object property. Additionally, each instance of this class is linked to a sensor to describe the agent that made the observation."@en ;
                             rdfs:label "Sleeping Duration Observation" ;
                             <http://www.w3.org/2004/02/skos/core#example> "A sleeping duration for the next irrigation is eight days."@en .


###  http://www.w3id.org/def/irrig#Soil30cmDepthDailyAverageMoistureObservation
:Soil30cmDepthDailyAverageMoistureObservation rdf:type owl:Class ;
                                              owl:equivalentClass [ owl:intersectionOf ( <http://www.w3id.org/def/caso#Observation>
                                                                                         [ rdf:type owl:Restriction ;
                                                                                           owl:onProperty <http://www.w3.org/ns/sosa/hasFeatureOfInterest> ;
                                                                                           owl:hasValue :featureOfInterest_soil30cmDepth
                                                                                         ]
                                                                                         [ rdf:type owl:Restriction ;
                                                                                           owl:onProperty <http://www.w3.org/ns/sosa/observedProperty> ;
                                                                                           owl:hasValue :observableProperty_soil30cmDepth_dailyAverageMoisture
                                                                                         ]
                                                                                       ) ;
                                                                    rdf:type owl:Class
                                                                  ] ;
                                              rdfs:subClassOf <http://www.w3id.org/def/caso#Observation> ;
                                              rdfs:comment "Soil30cmDepthDailyAverageMoistureObservation - A defined class that represents the act of carrying out a procedure (observation) to estimate the value of the daily average moisture property for the soil at 30 cm depth entity. The daily average moisture property is represented by the individual irrig:observableProperty_soil30cmDepth_dailyAverageMoisture. The soil at 30 cm depth entity is represented by the individual irrig:featureOfInterest_soil30cmDepth. Two necessary and sufficient conditions are defined: (1) All instances of this class are linked to the individual irrig:observableProperty_soil30cmDepth_dailyAverageMoisture via the sosa:observedProperty object property; (2) All instances of this class are linked to the individual irrig:featureOfInterest_soil30cmDepth via the sosa:hasFeatureOfInterest object property. Additionally, each instance of this class is linked to a sensor to describe the agent that made the observation."@en ;
                                              rdfs:label "Soil 30cm Depth Daily Average Moisture Observation"@en ;
                                              <http://www.w3.org/2004/02/skos/core#example> "A Soil30cmDepthDailyAverageMoistureObservation is computed by an aggregator."@en .


###  http://www.w3id.org/def/irrig#Soil30cmDepthMoistureObservation
:Soil30cmDepthMoistureObservation rdf:type owl:Class ;
                                  owl:equivalentClass [ owl:intersectionOf ( <http://www.w3id.org/def/caso#Observation>
                                                                             [ rdf:type owl:Restriction ;
                                                                               owl:onProperty <http://www.w3.org/ns/sosa/hasFeatureOfInterest> ;
                                                                               owl:hasValue :featureOfInterest_soil30cmDepth
                                                                             ]
                                                                             [ rdf:type owl:Restriction ;
                                                                               owl:onProperty <http://www.w3.org/ns/sosa/observedProperty> ;
                                                                               owl:hasValue :observableProperty_soil30cmDepth_moisture
                                                                             ]
                                                                           ) ;
                                                        rdf:type owl:Class
                                                      ] ;
                                  rdfs:subClassOf <http://www.w3id.org/def/caso#Observation> ;
                                  rdfs:comment "Soil30cmDepthDailyAverageMoistureObservation - A defined class that represents the act of carrying out a procedure (observation) to estimate the value of the moisture property for the soil at 30 cm depth entity. The daily average moisture property is represented by the individual irrig:observableProperty_soil30cmDepth_moisture. The soil at 30 cm depth entity is represented by the individual irrig:featureOfInterest_soil30cmDepth. Two necessary and sufficient conditions are defined: (1) All instances of this class are linked to the individual irrig:observableProperty_soil30cmDepth_moisture via the sosa:observedProperty object property; (2) All instances of this class are linked to the individual irrig:featureOfInterest_soil30cmDepth via the sosa:hasFeatureOfInterest object property. Additionally, each instance of this class is linked to a sensor to describe the agent that made the observation."@en ;
                                  rdfs:label "Soil 30cm Depth Moisture Observation"@en ;
                                  <http://www.w3.org/2004/02/skos/core#example> "A Soil30cmDepthMoistureObservation is made by a tensiometer placed at 30 cm depth in the soil."@en .


###  http://www.w3id.org/def/irrig#Soil60cmDepthDailyAverageMoistureObservation
:Soil60cmDepthDailyAverageMoistureObservation rdf:type owl:Class ;
                                              owl:equivalentClass [ owl:intersectionOf ( <http://www.w3id.org/def/caso#Observation>
                                                                                         [ rdf:type owl:Restriction ;
                                                                                           owl:onProperty <http://www.w3.org/ns/sosa/hasFeatureOfInterest> ;
                                                                                           owl:hasValue :featureOfInterest_soil60cmDepth
                                                                                         ]
                                                                                         [ rdf:type owl:Restriction ;
                                                                                           owl:onProperty <http://www.w3.org/ns/sosa/observedProperty> ;
                                                                                           owl:hasValue :observableProperty_soil60cmDepth_dailyAverageMoisture
                                                                                         ]
                                                                                       ) ;
                                                                    rdf:type owl:Class
                                                                  ] ;
                                              rdfs:subClassOf <http://www.w3id.org/def/caso#Observation> ;
                                              rdfs:comment "Soil60cmDepthDailyAverageMoistureObservation - A defined class that represents the act of carrying out a procedure (observation) to estimate the value of the daily average moisture property for the soil at 60 cm depth entity. The daily average moisture property is represented by the individual irrig:observableProperty_soil60cmDepth_dailyAverageMoisture. The soil at 60 cm depth entity is represented by the individual irrig:featureOfInterest_soil60cmDepth. Two necessary and sufficient conditions are defined: (1) All instances of this class are linked to the individual irrig:observableProperty_soil60cmDepth_dailyAverageMoisture via the sosa:observedProperty object property; (2) All instances of this class are linked to the individual irrig:featureOfInterest_soil60cmDepth via the sosa:hasFeatureOfInterest object property. Additionally, each instance of this class is linked to a sensor to describe the agent that made the observation."@en ;
                                              rdfs:label "Soil 60cm Depth Daily Average Moisture Observation"@en ;
                                              <http://www.w3.org/2004/02/skos/core#example> "A Soil60cmDepthAverageDailyMoistureObservation is made by an aggregator."@en .


###  http://www.w3id.org/def/irrig#Soil60cmDepthMoistureObservation
:Soil60cmDepthMoistureObservation rdf:type owl:Class ;
                                  owl:equivalentClass [ owl:intersectionOf ( <http://www.w3id.org/def/caso#Observation>
                                                                             [ rdf:type owl:Restriction ;
                                                                               owl:onProperty <http://www.w3.org/ns/sosa/hasFeatureOfInterest> ;
                                                                               owl:hasValue :featureOfInterest_soil60cmDepth
                                                                             ]
                                                                             [ rdf:type owl:Restriction ;
                                                                               owl:onProperty <http://www.w3.org/ns/sosa/observedProperty> ;
                                                                               owl:hasValue :observableProperty_soil60cmDepth_moisture
                                                                             ]
                                                                           ) ;
                                                        rdf:type owl:Class
                                                      ] ;
                                  rdfs:subClassOf <http://www.w3id.org/def/caso#Observation> ;
                                  rdfs:comment "Soil60cmDepthDailyAverageMoistureObservation - A defined class that represents the act of carrying out a procedure (observation) to estimate the value of the moisture property for the soil at 60 cm depth entity. The daily average moisture property is represented by the individual irrig:observableProperty_soil60cmDepth_moisture. The soil at 60 cm depth entity is represented by the individual irrig:featureOfInterest_soil60cmDepth. Two necessary and sufficient conditions are defined: (1) All instances of this class are linked to the individual irrig:observableProperty_soil60cmDepth_moisture via the sosa:observedProperty object property; (2) All instances of this class are linked to the individual irrig:featureOfInterest_soil60cmDepth via the sosa:hasFeatureOfInterest object property. Additionally, each instance of this class is linked to a sensor to describe the agent that made the observation."@en ;
                                  rdfs:label "Soil 60cm Depth Moisture Observation"@en ;
                                  <http://www.w3.org/2004/02/skos/core#example> "A Soil60cmDepthMoistureObservation is made by a tensiometer placed at 60 cm depth in the soil."@en .


###  http://www.w3id.org/def/irrig#StressProperty
:StressProperty rdf:type owl:Class ;
                rdfs:subClassOf <http://www.w3.org/ns/ssn/Property> ;
                rdfs:comment "StressProperty - Stress aspect of an entity, that is, the pressure inside the entity. The stress aspect of an entity is intrinsic and cannot exist without the entity. The stress quality should be expressed by a qualitative value such as a state or by a quantitative value."@en ;
                rdfs:label "Stress Property"@en ;
                <http://www.w3.org/2004/02/skos/core#example> "CropWaterNeed is a StressProperty representing the stress inside the plant when it needs extra water."@en .


###  http://www.w3id.org/def/irrig#TemperatureProperty
:TemperatureProperty rdf:type owl:Class ;
                     rdfs:subClassOf <http://www.w3.org/ns/ssn/Property> ;
                     rdfs:comment "TemperatureProperty - Temperature aspect of an entity. The temperature aspect of an entity is intrinsic and cannot exist without the entity. The temperature quality should be expressed by a qualitative value such as a state or by a quantitative value." ;
                     rdfs:label "Temperature Property" ;
                     <http://www.w3.org/2004/02/skos/core#example> "AirTemperature is a TemperatureProperty representing the temperature value of the air."@en .


###  https://w3id.org/def/saref4agri#Pluviometer
<https://w3id.org/def/saref4agri#Pluviometer> rdf:type owl:Class ;
                                              rdfs:subClassOf <https://w3id.org/saref#Sensor> ;
                                              rdfs:comment "A sensor that measures the rain fall."@en ;
                                              rdfs:label "Pluviometer"@en .


###  https://w3id.org/def/saref4agri#SoilTensiometer
<https://w3id.org/def/saref4agri#SoilTensiometer> rdf:type owl:Class ;
                                                  rdfs:subClassOf <https://w3id.org/saref#Sensor> ;
                                                  rdfs:comment "A sensor that measures the soil moisture."@en ;
                                                  rdfs:label "Soil Tensiometer"@en .


###  https://w3id.org/def/saref4agri#Thermometer
<https://w3id.org/def/saref4agri#Thermometer> rdf:type owl:Class ;
                                              rdfs:subClassOf <https://w3id.org/saref#Sensor> ;
                                              rdfs:comment "A sensor that measure weather conditions."@en ;
                                              rdfs:label "Thermometer"@en .


###  https://w3id.org/def/saref4agri#WateringValve
<https://w3id.org/def/saref4agri#WateringValve> rdf:type owl:Class ;
                                                rdfs:subClassOf <https://w3id.org/saref#Actuator> ;
                                                rdfs:comment "An actuator that open the water valve."@en ;
                                                rdfs:label "Watering Valve"@en .


#################################################################
#    Individuals
#################################################################

###  http://www.w3id.org/def/irrig#actuator_wateringValve_1
:actuator_wateringValve_1 rdf:type owl:NamedIndividual ,
                                   <https://w3id.org/def/saref4agri#WateringValve> ;
                          rdfs:comment "Actuator_wateringValve_1 - An actuator n°1 that controls the valve of water."@en ;
                          rdfs:label "Actuator Watering  Valve 01 Soil Moisture" .


###  http://www.w3id.org/def/irrig#boundary_rain_quantity_high
:boundary_rain_quantity_high rdf:type owl:NamedIndividual ,
                                      :RainIntensityBoundary ;
                             rdfs:comment """Boundary_rain_quantity_high - a boundary line of division between two states of Rain Intensity: Heavy and Moderate.

In the example of Arvalis' dataset, the value of boundary rain quantity high is 40mm.""" ;
                             rdfs:label "Boundary Rain Quantity High" .


###  http://www.w3id.org/def/irrig#boundary_rain_quantity_low
:boundary_rain_quantity_low rdf:type owl:NamedIndividual ,
                                     :RainIntensityBoundary ;
                            rdfs:comment """Boundary_rain_quantity_low  - a boundary line of division between two states of Rain Intensity: Moderate and Light.

In the example of Arvalis' dataset, the value of boundary rain quantity low is 10mm.""" ;
                            rdfs:label "Boundary Rain Quantity Low" .


###  http://www.w3id.org/def/irrig#boundary_rain_quantity_maximum
:boundary_rain_quantity_maximum rdf:type owl:NamedIndividual ,
                                         :RainIntensityBoundary ;
                                rdfs:comment """Boundary_rain_quantity_maximum - a boundary line represents the maximal value that rain quantity cannot surpass.

In the example of Arvalis' dataset, the value of boundary rain quantity maximum is 90.0mm (even more than the word record which is 71.8mm)""" ;
                                rdfs:label "Boundary Rain Quantity Maximum" .


###  http://www.w3id.org/def/irrig#boundary_rain_quantity_minimum
:boundary_rain_quantity_minimum rdf:type owl:NamedIndividual ,
                                         :RainIntensityBoundary ;
                                rdfs:comment """Boundary_rain_quantity_maximum - a boundary line represents the minimal value that rain quantity cannot below.

In the example of Arvalis' dataset, the value of boundary rain quantity minimum is 0mm.""" ;
                                rdfs:label "Boundary Rain Quantity Minimum" .


###  http://www.w3id.org/def/irrig#boundary_rootZone_tension_average
:boundary_rootZone_tension_average rdf:type owl:NamedIndividual ,
                                            :RootZoneMoistureLevelBoundary ;
                                   rdfs:comment """Boundary_rootZone_tension_average - a boundary line of division between two states of RootZone MoistureLevel: Low and Average.

In the example of Arvalis' dataset, the value of boundary rootzone tension average is 140.0 cbar or 1400.0 mbar.""" ;
                                   rdfs:label "Boundary RootZone Tension Average" .


###  http://www.w3id.org/def/irrig#boundary_rootZone_tension_high
:boundary_rootZone_tension_high rdf:type owl:NamedIndividual ,
                                         :RootZoneMoistureLevelBoundary ;
                                rdfs:comment """Boundary_rootZone_tension_high - a boundary line of division between two states of RootZone MoistureLevel: Average and High.

In the example of Arvalis' dataset, the value of boundary rootzone tension high is 120.0 cbar or 1200.0 mbar.""" ;
                                rdfs:label "Boundary RootZone Tension High" .


###  http://www.w3id.org/def/irrig#boundary_rootZone_tension_low
:boundary_rootZone_tension_low rdf:type owl:NamedIndividual ,
                                        :RootZoneMoistureLevelBoundary ;
                               rdfs:comment """Boundary_rootZone_tension_low - a boundary line of division between two states of RootZone MoistureLevel: VeryLow and Low.

In the example of Arvalis' dataset, the value of boundary rootzone tension low is 150.0 cbar or 1500.0 mbar.""" ;
                               rdfs:label "Boundary RootZone Tension Low" .


###  http://www.w3id.org/def/irrig#boundary_rootZone_tension_maximum
:boundary_rootZone_tension_maximum rdf:type owl:NamedIndividual ,
                                            :RootZoneMoistureLevelBoundary ;
                                   rdfs:comment """Boundary_rootZone_moistureLevel_maximum - a boundary line represents the maximal value that RootZone Tension cannot surpass.

In the example of Arvalis' dataset, the value of boundary rootzone tension maximum is 301cbar or 3010 mbar (even more than the possible value of Watermark can evalute which is 300 cbar).""" ;
                                   rdfs:label "Boundary RootZone Tension Maximum" .


###  http://www.w3id.org/def/irrig#boundary_rootZone_tension_minimum
:boundary_rootZone_tension_minimum rdf:type owl:NamedIndividual ,
                                            :RootZoneMoistureLevelBoundary ;
                                   rdfs:comment """Boundary_rootZone_moistureLevel_minimum - a boundary line represents the minimal value that RootZone Tension cannot below.

In the example of Arvalis' dataset, the value of boundary rootzone tension minimum is 0 cbar or 0 mbar.""" ;
                                   rdfs:label "Boundary RootZone Tension Minimum" .


###  http://www.w3id.org/def/irrig#boundary_rootZone_tension_saturation
:boundary_rootZone_tension_saturation rdf:type owl:NamedIndividual ,
                                               :RootZoneMoistureLevelBoundary ;
                                      rdfs:comment """Boundary_rootZone_tension_saturation - a boundary line of division between two states of RootZone MoistureLevel: VeryHigh and Saturated.

In the example of Arvalis' dataset, the value of boundary rootzone tension saturation is 10.0 cbar or 100.0 mbar.""" ;
                                      rdfs:label "Boundary RootZone Tension Saturation" .


###  http://www.w3id.org/def/irrig#boundary_rootZone_tension_veryHigh
:boundary_rootZone_tension_veryHigh rdf:type owl:NamedIndividual ,
                                             :RootZoneMoistureLevelBoundary ;
                                    rdfs:comment """Boundary_rootZone_tension_veryHigh - a boundary line of division between two states of RootZone MoistureLevel: High and VeryHigh.

In the example of Arvalis' dataset, the value of boundary rootzone tension very high is 70.0 cbar or 700.0 mbar.""" ;
                                    rdfs:label "Boundary RootZone Tension VeryHigh" .


###  http://www.w3id.org/def/irrig#boundary_rootZone_tension_veryLow
:boundary_rootZone_tension_veryLow rdf:type owl:NamedIndividual ,
                                            :RootZoneMoistureLevelBoundary ;
                                   rdfs:comment """Boundary_rootZone_tension_veryLow - a boundary line of division between two states of RootZone MoistureLevel: Dry and VeryLow.

In the example of Arvalis' dataset, the value of boundary rootzone tension very low is 160.0 cbar or 1600.0 mbar.""" ;
                                   rdfs:label "Boundary RootZone Tension VeryLow" .


###  http://www.w3id.org/def/irrig#featureOfInterest_air
:featureOfInterest_air rdf:type owl:NamedIndividual ,
                                <http://www.w3.org/ns/sosa/FeatureOfInterest> ;
                       <http://www.w3.org/ns/ssn/hasProperty> :observableProperty_air_dailyMaxTemperature ,
                                                              :observableProperty_air_dailyMinTemperature ,
                                                              :observableProperty_air_temperature ;
                       rdfs:comment "FeatureOfInterest_air - an instance of the class sosa:FeatureOfInterest that represents air." ;
                       rdfs:label "Feature Of Interest Air" .


###  http://www.w3id.org/def/irrig#featureOfInterest_crop
:featureOfInterest_crop rdf:type owl:NamedIndividual ,
                                 <http://www.w3.org/ns/sosa/FeatureOfInterest> ;
                        <http://www.w3.org/ns/ssn/hasProperty> :observableProperty_crop_growth ,
                                                               :observableProperty_crop_waterNeed ;
                        rdfs:comment """FeatureOfInterest_crop - an instance of the class sosa:FeatureOfInterest that represents crop. The crop needs to be irrigated. 

In the example of Arvalis' dataset, the crop is maize that growth in an Arvalis' plot in 2013.""" ;
                        rdfs:label "Feature Of Interest Crop" .


###  http://www.w3id.org/def/irrig#featureOfInterest_delay
:featureOfInterest_delay rdf:type owl:NamedIndividual ,
                                  <http://www.w3.org/ns/sosa/FeatureOfInterest> ;
                         <http://www.w3.org/ns/ssn/hasProperty> :observableProperty_delayDuration ;
                         rdfs:comment "FeatureOfInterest_delay - an instance of the class sosa:FeatureOfInterest that represents delay phenomenon."@en ;
                         rdfs:label "Feature Of Interest Delay" .


###  http://www.w3id.org/def/irrig#featureOfInterest_rain
:featureOfInterest_rain rdf:type owl:NamedIndividual ,
                                 <http://www.w3.org/ns/sosa/FeatureOfInterest> ;
                        <http://www.w3.org/ns/ssn/hasProperty> :observableProperty_rain_dailyTotalQuantity ,
                                                               :observableProperty_rain_intensity ,
                                                               :observableProperty_rain_quantity ;
                        rdfs:comment "FeatureOfInterest_rain - an instance of the class sosa:FeatureOfInterest that represents rain." ;
                        rdfs:label "Feature Of Interest Rain" .


###  http://www.w3id.org/def/irrig#featureOfInterest_rootZone
:featureOfInterest_rootZone rdf:type owl:NamedIndividual ,
                                     <http://www.w3.org/ns/sosa/FeatureOfInterest> ;
                            <http://www.w3.org/ns/ssn/hasProperty> :observableProperty_rootZone_dailyAverageMoisture ,
                                                                   :observableProperty_rootZone_moistureLevel ;
                            rdfs:comment "FeatureOfInterest_rootzone - an instance of the class sosa:FeatureOfInterest that represents rootzone soil of a plant." ;
                            rdfs:label "Feature Of Interest Root Zone" .


###  http://www.w3id.org/def/irrig#featureOfInterest_sleeping
:featureOfInterest_sleeping rdf:type owl:NamedIndividual ,
                                     <http://www.w3.org/ns/sosa/FeatureOfInterest> ;
                            <http://www.w3.org/ns/ssn/hasProperty> :observableProperty_sleepingDuration ;
                            rdfs:comment "FeatureOfInterest_sleeping - an instance of the class sosa:FeatureOfInterest that represents sleeping phenomenon."@en ;
                            rdfs:label "Feature Of Interest Sleeping" .


###  http://www.w3id.org/def/irrig#featureOfInterest_soil30cmDepth
:featureOfInterest_soil30cmDepth rdf:type owl:NamedIndividual ,
                                          <http://www.w3.org/ns/sosa/FeatureOfInterest> ;
                                 <http://www.w3.org/ns/ssn/hasProperty> :observableProperty_soil30cmDepth_dailyAverageMoisture ,
                                                                        :observableProperty_soil30cmDepth_moisture ;
                                 rdfs:comment "FeatureOfInterest_soil30cmDepth - an instance of the class sosa:FeatureOfInterest that represents soil at 30cm depth." ;
                                 rdfs:label "Feature Of Interest Soil at 30cm Depth" .


###  http://www.w3id.org/def/irrig#featureOfInterest_soil60cmDepth
:featureOfInterest_soil60cmDepth rdf:type owl:NamedIndividual ,
                                          <http://www.w3.org/ns/sosa/FeatureOfInterest> ;
                                 <http://www.w3.org/ns/ssn/hasProperty> :observableProperty_soil60cmDepth_dailyAverageMoisture ,
                                                                        :observableProperty_soil60cmDepth_moisture ;
                                 rdfs:comment "FeatureOfInterest_soil30cmDepth - an instance of the class sosa:FeatureOfInterest that represents soil at 60cm depth." ;
                                 rdfs:label "Feature Of Interest Soil at 60cm Depth" .


###  http://www.w3id.org/def/irrig#observableProperty_air_dailyMaxTemperature
:observableProperty_air_dailyMaxTemperature rdf:type owl:NamedIndividual ,
                                                     <http://www.w3.org/ns/sosa/ObservableProperty> ,
                                                     :TemperatureProperty ;
                                            rdfs:comment "ObservableProperty_air_dailyMaxTemperature - an instance of the class irrig:TemperatureProperty and sosa:ObservableProperty that represents the observable property of max temperature per day of an air feature of interest." ;
                                            rdfs:label "Observable Property Air Daily Max Temperature" .


###  http://www.w3id.org/def/irrig#observableProperty_air_dailyMinTemperature
:observableProperty_air_dailyMinTemperature rdf:type owl:NamedIndividual ,
                                                     <http://www.w3.org/ns/sosa/ObservableProperty> ,
                                                     :TemperatureProperty ;
                                            rdfs:comment "ObservableProperty_air_dailyMinTemperature - an instance of the class irrig:TemperatureProperty and sosa:ObservableProperty that represents the observable property of min temperature per day of an air feature of interest." ;
                                            rdfs:label "Observable Property Air Daily Min Temperature" .


###  http://www.w3id.org/def/irrig#observableProperty_air_temperature
:observableProperty_air_temperature rdf:type owl:NamedIndividual ,
                                             <http://www.w3.org/ns/sosa/ObservableProperty> ,
                                             :TemperatureProperty ;
                                    rdfs:comment "ObservableProperty_air_temperature - an instance of the class irrig:TemperatureProperty and sosa:ObservableProperty that represents the observable property of temperature of an air feature of interest." ;
                                    rdfs:label "Observable Property Air Temperature" .


###  http://www.w3id.org/def/irrig#observableProperty_crop_growth
:observableProperty_crop_growth rdf:type owl:NamedIndividual ,
                                         <http://www.w3id.org/def/caso#Property> ,
                                         :GrowthProperty ;
                                <http://www.w3id.org/def/caso#hasState> :state_crop_growth_init ,
                                                                        :state_crop_growth_r1 ,
                                                                        :state_crop_growth_r1d15 ,
                                                                        :state_crop_growth_r5 ,
                                                                        :state_crop_growth_r5hg45 ,
                                                                        :state_crop_growth_v2 ,
                                                                        :state_crop_growth_v7 ,
                                                                        :state_crop_growth_v7d20 ;
                                rdfs:comment "ObservableProperty_crop_growth - an instance of the class irrig:GrowthProperty and caso:Property that represents the observable property of growth of a crop feature of interest." ;
                                rdfs:label "Observable Property Crop Growth" .


###  http://www.w3id.org/def/irrig#observableProperty_crop_stage
:observableProperty_crop_stage rdf:type owl:NamedIndividual ,
                                        <http://www.w3id.org/def/caso#Property> ,
                                        :GrowthProperty ;
                               rdfs:comment "ObservableProperty_crop_stage - an instance of the class irrig:GrowthProperty and caso:Property that represents the stage observable property of a crop feature of interest." ;
                               rdfs:label "Observable Property Crop Stage" .


###  http://www.w3id.org/def/irrig#observableProperty_crop_waterNeed
:observableProperty_crop_waterNeed rdf:type owl:NamedIndividual ,
                                            <http://www.w3id.org/def/caso#Property> ,
                                            :StressProperty ;
                                   <http://www.w3id.org/def/caso#hasState> :state_crop_waterNeed_init ,
                                                                           :state_crop_waterNeed_no ,
                                                                           :state_crop_waterNeed_unavailable ,
                                                                           :state_crop_waterNeed_yes ;
                                   rdfs:comment "ObservableProperty_crop_waterNeed - an instance of the class irrig:StressProperty and caso:Property that represents the observable property of water need of an crop feature of interest." ;
                                   rdfs:label "Observable Property Crop Water Need" .


###  http://www.w3id.org/def/irrig#observableProperty_delayDuration
:observableProperty_delayDuration rdf:type owl:NamedIndividual ,
                                           <http://www.w3id.org/def/caso#Property> ;
                                  rdfs:comment "Number of days that an watering is delayed."@en ;
                                  rdfs:label "Observable Property Irrigation Delay"@en .


###  http://www.w3id.org/def/irrig#observableProperty_rain_dailyTotalQuantity
:observableProperty_rain_dailyTotalQuantity rdf:type owl:NamedIndividual ,
                                                     <http://www.w3.org/ns/sosa/ObservableProperty> ,
                                                     :AmountProperty ;
                                            rdfs:comment "ObservableProperty_rain_dailyTotalQuantity - an instance of the class irrig:AmountProperty and sosa:ObservableProperty that represents the observable property of total quantity per day of a rain feature of interest." ;
                                            rdfs:label "Observable Property Rain Daily Total Quantity" .


###  http://www.w3id.org/def/irrig#observableProperty_rain_intensity
:observableProperty_rain_intensity rdf:type owl:NamedIndividual ,
                                            <http://www.w3id.org/def/caso#Property> ,
                                            :IntensityProperty ;
                                   <http://www.w3id.org/def/caso#hasState> :state_rain_intensity_heavy ,
                                                                           :state_rain_intensity_init ,
                                                                           :state_rain_intensity_light ,
                                                                           :state_rain_intensity_moderate ;
                                   rdfs:comment "ObservableProperty_rain_intensity - an instance of the class irrig:IntensityProperty and caso:Property that represents the intensity observable property of a rain feature of interest." ;
                                   rdfs:label "Observable Property Rain Intensity" .


###  http://www.w3id.org/def/irrig#observableProperty_rain_quantity
:observableProperty_rain_quantity rdf:type owl:NamedIndividual ,
                                           <http://www.w3.org/ns/sosa/ObservableProperty> ,
                                           :AmountProperty ;
                                  rdfs:comment "ObservableProperty_rain_quantity - an instance of the class irrig:AmountProperty and sosa:ObservableProperty that represents the quantity observable property of a rain feature of interest." ;
                                  rdfs:label "Observable Property Rain Quantity" .


###  http://www.w3id.org/def/irrig#observableProperty_rootZone_dailyAverageMoisture
:observableProperty_rootZone_dailyAverageMoisture rdf:type owl:NamedIndividual ,
                                                           <http://www.w3.org/ns/sosa/ObservableProperty> ,
                                                           :MoistureProperty ;
                                                  rdfs:comment "ObservableProperty_rootZone_dailyAverageMoisture - an instance of the class irrig:MoistureProperty and sosa:ObservableProperty that represents the observable property of average moisture per day of a root zone feature of interest." ;
                                                  rdfs:label "Observable Property Root Zone Daily Average Moisture" .


###  http://www.w3id.org/def/irrig#observableProperty_rootZone_moistureLevel
:observableProperty_rootZone_moistureLevel rdf:type owl:NamedIndividual ,
                                                    <http://www.w3id.org/def/caso#Property> ,
                                                    :MoistureProperty ;
                                           <http://www.w3id.org/def/caso#hasState> :state_rootZone_moistureLevel_average ,
                                                                                   :state_rootZone_moistureLevel_dry ,
                                                                                   :state_rootZone_moistureLevel_high ,
                                                                                   :state_rootZone_moistureLevel_init ,
                                                                                   :state_rootZone_moistureLevel_low ,
                                                                                   :state_rootZone_moistureLevel_saturated ,
                                                                                   :state_rootZone_moistureLevel_veryHigh ,
                                                                                   :state_rootZone_moistureLevel_veryLow ;
                                           rdfs:comment "ObservableProperty_rootZone_moistureLevel - an instance of the class irrig:MoistureProperty and caso:Property that represents the observable property of moisture level of a root zone feature of interest." ;
                                           rdfs:label "Observable Property Root Zone Moisture Level" .


###  http://www.w3id.org/def/irrig#observableProperty_sleepingDuration
:observableProperty_sleepingDuration rdf:type owl:NamedIndividual ,
                                              <http://www.w3id.org/def/caso#Property> ;
                                     rdfs:comment "Number of days that the system is waiting until the next irrigation."@en ;
                                     rdfs:label "Observable Property Sleeping Duration" .


###  http://www.w3id.org/def/irrig#observableProperty_soil30cmDepth_dailyAverageMoisture
:observableProperty_soil30cmDepth_dailyAverageMoisture rdf:type owl:NamedIndividual ,
                                                                <http://www.w3.org/ns/sosa/ObservableProperty> ,
                                                                :MoistureProperty ;
                                                       rdfs:comment "ObservableProperty_soil30cmDepth_dailyAverageMoisture - an instance of the class irrig:MoistureProperty and sosa:ObservableProperty that represents the observable property of average moisture per day of a soil 30cm depth feature of interest." ;
                                                       rdfs:label "Observable Property Soil 30cm Depth Daily Average Moisture" .


###  http://www.w3id.org/def/irrig#observableProperty_soil30cmDepth_moisture
:observableProperty_soil30cmDepth_moisture rdf:type owl:NamedIndividual ,
                                                    <http://www.w3.org/ns/sosa/ObservableProperty> ,
                                                    :MoistureProperty ;
                                           rdfs:comment "ObservableProperty_soil30cmDepth_moisture - an instance of the class irrig:MoistureProperty and sosa:ObservableProperty that represents the observable property of moisture of a soil 30cm depth feature of interest." ;
                                           rdfs:label "Observable Property Soil 30cm Depth Moisture" .


###  http://www.w3id.org/def/irrig#observableProperty_soil60cmDepth_dailyAverageMoisture
:observableProperty_soil60cmDepth_dailyAverageMoisture rdf:type owl:NamedIndividual ,
                                                                <http://www.w3.org/ns/sosa/ObservableProperty> ,
                                                                :MoistureProperty ;
                                                       rdfs:comment "ObservableProperty_soil60cmDepth_dailyAverageMoisture - an instance of the class irrig:MoistureProperty and sosa:ObservableProperty that represents the observable property of average moisture per day of a soil 60cm depth feature of interest." ;
                                                       rdfs:label "Observable Property Soil 60cm Depth Daily Average Moisture" .


###  http://www.w3id.org/def/irrig#observableProperty_soil60cmDepth_moisture
:observableProperty_soil60cmDepth_moisture rdf:type owl:NamedIndividual ,
                                                    <http://www.w3.org/ns/sosa/ObservableProperty> ,
                                                    :MoistureProperty ;
                                           rdfs:comment "ObservableProperty_soil60cmDepth_moisture - an instance of the class irrig:MoistureProperty and sosa:ObservableProperty that represents the observable property of moisture of a soil 60cm depth feature of interest." ;
                                           rdfs:label "Observable Property Soil 60cm Depth Moisture" .


###  http://www.w3id.org/def/irrig#pluviometer_1
:pluviometer_1 rdf:type owl:NamedIndividual ,
                        <https://w3id.org/def/saref4agri#Pluviometer> ;
               rdfs:comment "Pluviometer_1 - a pluviometer measures the rain quantity n° 01." ;
               rdfs:label "Pluviometer 1" .


###  http://www.w3id.org/def/irrig#pluviometer_2
:pluviometer_2 rdf:type owl:NamedIndividual ,
                        <https://w3id.org/def/saref4agri#Pluviometer> ;
               rdfs:comment "Pluviometer_2 - a pluviometer measures the rain quantity n° 02." ;
               rdfs:label "Pluviometer 2" .


###  http://www.w3id.org/def/irrig#soilTensiometer_1_30cm
:soilTensiometer_1_30cm rdf:type owl:NamedIndividual ,
                                 <https://w3id.org/def/saref4agri#SoilTensiometer> ;
                        rdfs:comment "SoilTensiometer_1_30cm - a soil tensiometer measures the moisture at 30 cm depth n° 01." ;
                        rdfs:label "Soil Tensiometer 1 at 30cm Depth" .


###  http://www.w3id.org/def/irrig#soilTensiometer_2_30cm
:soilTensiometer_2_30cm rdf:type owl:NamedIndividual ,
                                 <https://w3id.org/def/saref4agri#SoilTensiometer> ;
                        rdfs:comment "SoilTensiometer_2_30cm - a soil tensiometer measures the moisture at 30 cm depth n° 02." ;
                        rdfs:label "Soil Tensiometer 2 at 30cm Depth" .


###  http://www.w3id.org/def/irrig#soilTensiometer_3_30cm
:soilTensiometer_3_30cm rdf:type owl:NamedIndividual ,
                                 <https://w3id.org/def/saref4agri#SoilTensiometer> ;
                        rdfs:comment "SoilTensiometer_3_30cm - a soil tensiometer measures the moisture at 30 cm depth n° 03." ;
                        rdfs:label "Soil Tensiometer 3 at 30cm Depth" .


###  http://www.w3id.org/def/irrig#soilTensiometer_4_60cm
:soilTensiometer_4_60cm rdf:type owl:NamedIndividual ,
                                 <https://w3id.org/def/saref4agri#SoilTensiometer> ;
                        rdfs:comment "SoilTensiometer_4_60cm - a soil tensiometer measures the moisture at 60 cm depth n° 04." ;
                        rdfs:label "Soil Tensiometer 4 at 60cm Depth" .


###  http://www.w3id.org/def/irrig#soilTensiometer_5_60cm
:soilTensiometer_5_60cm rdf:type owl:NamedIndividual ,
                                 <https://w3id.org/def/saref4agri#SoilTensiometer> ;
                        rdfs:comment "SoilTensiometer_5_60cm - a soil tensiometer measures the moisture at 60 cm depth n° 05." ;
                        rdfs:label "Soil Tensiometer 5 at 60cm Depth" .


###  http://www.w3id.org/def/irrig#soilTensiometer_6_60cm
:soilTensiometer_6_60cm rdf:type owl:NamedIndividual ,
                                 <https://w3id.org/def/saref4agri#SoilTensiometer> ;
                        rdfs:comment "SoilTensiometer_6_60cm - a soil tensiometer measures the moisture at 60 cm depth n° 06." ;
                        rdfs:label "Soil Tensiometer 6 at 60cm Depth" .


###  http://www.w3id.org/def/irrig#state_crop_growth_init
:state_crop_growth_init rdf:type owl:NamedIndividual ,
                                 :CropGrowthState ;
                        rdfs:comment "State_crop_growth_init - an instance of the class caso:State that represents the state of crop growth is temporary undefined." ;
                        rdfs:label "State Crop Growth Init" .


###  http://www.w3id.org/def/irrig#state_crop_growth_r1
:state_crop_growth_r1 rdf:type owl:NamedIndividual ,
                               :CropGrowthState ;
                      <http://www.w3id.org/def/caso#greaterThan> :state_crop_growth_v7d20 ;
                      <http://www.w3id.org/def/caso#lesserThan> :state_crop_growth_r1d15 ;
                      rdfs:comment "State_crop_growth_r1 - an instance of the class caso:State that represents the crop after reaching the “silking” stage. This stage is also named R1." ;
                      rdfs:label "State Crop Growth R1" .


###  http://www.w3id.org/def/irrig#state_crop_growth_r1d15
:state_crop_growth_r1d15 rdf:type owl:NamedIndividual ,
                                  :CropGrowthState ;
                         <http://www.w3id.org/def/caso#greaterThan> :state_crop_growth_r1 ;
                         <http://www.w3id.org/def/caso#lesserThan> :state_crop_growth_r5 ;
                         rdfs:comment "State_crop_growth_r1d15 - an instance of the class caso:State that represents the crop 15 days after reaching the “silking” stage." ;
                         rdfs:label "State Crop Growth R1d15" .


###  http://www.w3id.org/def/irrig#state_crop_growth_r5
:state_crop_growth_r5 rdf:type owl:NamedIndividual ,
                               :CropGrowthState ;
                      <http://www.w3id.org/def/caso#greaterThan> :state_crop_growth_r1d15 ;
                      <http://www.w3id.org/def/caso#lesserThan> :state_crop_growth_r5hg45 ;
                      rdfs:comment "State_crop_growth_r5 - an instance of the class caso:State that represents the crop after reaching the “dent stage within kernel containing 50% moisture”. This stage is also named R5" ;
                      rdfs:label "State Crop Growth R5" .


###  http://www.w3id.org/def/irrig#state_crop_growth_r5hg45
:state_crop_growth_r5hg45 rdf:type owl:NamedIndividual ,
                                   :CropGrowthState ;
                          <http://www.w3id.org/def/caso#greaterThan> :state_crop_growth_r5 ;
                          rdfs:comment "State_crop_growth_r5hg45 - an instance of the class caso:State that represents the crop after reaching the “dent stage within kernel containing 45% moisture”." ;
                          rdfs:label "State Crop Growth R5hg45" .


###  http://www.w3id.org/def/irrig#state_crop_growth_v2
:state_crop_growth_v2 rdf:type owl:NamedIndividual ,
                               :CropGrowthState ;
                      <http://www.w3id.org/def/caso#lesserThan> :state_crop_growth_v7 ;
                      rdfs:comment "State_crop_growth_v2 - an instance of the class caso:State that represents the crop after reaching the crop stage “5 leaves”, also named V2." ;
                      rdfs:label "State Crop Growth V2" .


###  http://www.w3id.org/def/irrig#state_crop_growth_v7
:state_crop_growth_v7 rdf:type owl:NamedIndividual ,
                               :CropGrowthState ;
                      <http://www.w3id.org/def/caso#greaterThan> :state_crop_growth_v2 ;
                      <http://www.w3id.org/def/caso#lesserThan> :state_crop_growth_v7d20 ;
                      rdfs:comment "State_crop_growth_v7 - an instance of the class caso:State that represents the crop after reaching the crop stage “10 leaves”, also named V7." ;
                      rdfs:label "State Crop Growth V7" .


###  http://www.w3id.org/def/irrig#state_crop_growth_v7d20
:state_crop_growth_v7d20 rdf:type owl:NamedIndividual ,
                                  :CropGrowthState ;
                         <http://www.w3id.org/def/caso#greaterThan> :state_crop_growth_v7 ;
                         <http://www.w3id.org/def/caso#lesserThan> :state_crop_growth_r1 ;
                         rdfs:comment "State_crop_growth_v7d20 - an instance of the class caso:State that represents the crop 20 days after reaching the stage “10 leaves”." ;
                         rdfs:label "State Crop Growth V7d20" .


###  http://www.w3id.org/def/irrig#state_crop_waterNeed_init
:state_crop_waterNeed_init rdf:type owl:NamedIndividual ,
                                    :CropWaterNeedState ;
                           rdfs:comment "State_crop_waterNeed_init - an instance of the class caso:State that represents the state of crop water need is temporary undefined." ;
                           rdfs:label "State Crop Water Need Init" .


###  http://www.w3id.org/def/irrig#state_crop_waterNeed_no
:state_crop_waterNeed_no rdf:type owl:NamedIndividual ,
                                  :CropWaterNeedState ;
                         rdfs:comment "State_crop_waterNeed_no - an instance of the class caso:State that represents the crop does not need water." ;
                         rdfs:label "State Crop Water Need No" .


###  http://www.w3id.org/def/irrig#state_crop_waterNeed_notApplicable
:state_crop_waterNeed_notApplicable rdf:type owl:NamedIndividual ,
                                             :CropWaterNeedState ;
                                    rdfs:comment "State_crop_waterNeed_notApplicable - an instance of the class caso:State that represents the state of crop water need has not been evaluated yet." ;
                                    rdfs:label "State Crop Water Need Not Applicable" .


###  http://www.w3id.org/def/irrig#state_crop_waterNeed_unavailable
:state_crop_waterNeed_unavailable rdf:type owl:NamedIndividual ,
                                           :CropWaterNeedState ;
                                  rdfs:comment "State_crop_waterNeed_unavailable - an instance of the class caso:State that represents the crop may need water soon." ;
                                  rdfs:label "State Crop Water Need Unavailable" .


###  http://www.w3id.org/def/irrig#state_crop_waterNeed_yes
:state_crop_waterNeed_yes rdf:type owl:NamedIndividual ,
                                   :CropWaterNeedState ;
                          rdfs:comment "State_crop_waterNeed_yes - an instance of the class caso:State that represents the crop needs water." ;
                          rdfs:label "State Crop Water Need Yes" .


###  http://www.w3id.org/def/irrig#state_rain_intensity_heavy
:state_rain_intensity_heavy rdf:type owl:NamedIndividual ,
                                     :RainIntensityState ;
                            <http://www.w3id.org/def/caso#greaterThan> :state_rain_intensity_moderate ;
                            rdfs:comment """State_rain_intensity_heavy - an instance of the class caso:State that represents the rain intensity is heavy.

In the example of Arvalis' dataset, this RainIntensity property reaches this state the open upper boundary is RQ_maximum and the close lower boundary is RQ_high.""" ;
                            rdfs:label "State Rain Intensity Heavy" .


###  http://www.w3id.org/def/irrig#state_rain_intensity_init
:state_rain_intensity_init rdf:type owl:NamedIndividual ,
                                    :RainIntensityState ;
                           rdfs:comment "State_rain_intensity_init - an instance of the class caso:State that represents the rain intensity is temporary undefined." ;
                           rdfs:label "State Rain Intensity Init" .


###  http://www.w3id.org/def/irrig#state_rain_intensity_light
:state_rain_intensity_light rdf:type owl:NamedIndividual ,
                                     :RainIntensityState ;
                            <http://www.w3id.org/def/caso#lesserThan> :state_rain_intensity_moderate ;
                            rdfs:comment """State_rain_intensity_light - an instance of the class caso:State that represents the rain intensity is light.

In the example of Arvalis' dataset, this RainIntensity property reaches this state the open upper boundary is RQ_low and the close lower boundary is RQ_minimum.""" ;
                            rdfs:label "State Rain Intensity Light" .


###  http://www.w3id.org/def/irrig#state_rain_intensity_moderate
:state_rain_intensity_moderate rdf:type owl:NamedIndividual ,
                                        :RainIntensityState ;
                               <http://www.w3id.org/def/caso#greaterThan> :state_rain_intensity_light ;
                               <http://www.w3id.org/def/caso#lesserThan> :state_rain_intensity_heavy ;
                               rdfs:comment """State_rain_intensity_moderate - an instance of the class caso:State that represents the rain intensity is moderate.

In the example of Arvalis' dataset, this RainIntensity property reaches this state the open upper boundary is RQ_high and the close lower boundary is RQ_low.""" ;
                               rdfs:label "State Rain Intensity Moderate" .


###  http://www.w3id.org/def/irrig#state_rootZone_moistureLevel_average
:state_rootZone_moistureLevel_average rdf:type owl:NamedIndividual ,
                                               :RootZoneMoistureLevelState ;
                                      <http://www.w3id.org/def/caso#greaterThan> :state_rootZone_moistureLevel_low ;
                                      <http://www.w3id.org/def/caso#lesserThan> :state_rootZone_moistureLevel_high ;
                                      rdfs:comment """State_rootZone_moistureLevel_average - an instance of the class caso:State that represents the root zone moisture level is at the average state.

In the example of Arvalis' dataset, this RootZoneMoistureLevel property reaches this state the open upper boundary is ST_average and the close lower boundary is ST_high.""" ;
                                      rdfs:label "State Root Zone Moisture Level Average" .


###  http://www.w3id.org/def/irrig#state_rootZone_moistureLevel_dry
:state_rootZone_moistureLevel_dry rdf:type owl:NamedIndividual ,
                                           :RootZoneMoistureLevelState ;
                                  <http://www.w3id.org/def/caso#lesserThan> :state_rootZone_moistureLevel_veryLow ;
                                  rdfs:comment """State_rootZone_moistureLevel_dry - an instance of the class caso:State that represents the root zone moisture level is at the dry state.

In the example of Arvalis' dataset, this RootZoneMoistureLevel property reaches this state the open upper boundary is ST_maximum and the close lower boundary is ST_very_low.""" ;
                                  rdfs:label "State Root Zone Moisture Level Dry" .


###  http://www.w3id.org/def/irrig#state_rootZone_moistureLevel_high
:state_rootZone_moistureLevel_high rdf:type owl:NamedIndividual ,
                                            :RootZoneMoistureLevelState ;
                                   <http://www.w3id.org/def/caso#greaterThan> :state_rootZone_moistureLevel_average ;
                                   <http://www.w3id.org/def/caso#lesserThan> :state_rootZone_moistureLevel_veryHigh ;
                                   rdfs:comment """State_rootZone_moistureLevel_high - an instance of the class caso:State that represents the root zone moisture level is at the high state.

In the example of Arvalis' dataset, this RootZoneMoistureLevel property reaches this state the open upper boundary is ST_high and the close lower boundary is ST_very_high.""" ;
                                   rdfs:label "State Root Zone Moisture Level High" .


###  http://www.w3id.org/def/irrig#state_rootZone_moistureLevel_init
:state_rootZone_moistureLevel_init rdf:type owl:NamedIndividual ,
                                            :RootZoneMoistureLevelState ;
                                   rdfs:comment "State_rootZone_moistureLevel_init - an instance of the class caso:State that represents the root zone moisture level is temporary undefined." ;
                                   rdfs:label "State Root Zone Moisture Level Init" .


###  http://www.w3id.org/def/irrig#state_rootZone_moistureLevel_low
:state_rootZone_moistureLevel_low rdf:type owl:NamedIndividual ,
                                           :RootZoneMoistureLevelState ;
                                  <http://www.w3id.org/def/caso#greaterThan> :state_rootZone_moistureLevel_veryLow ;
                                  <http://www.w3id.org/def/caso#lesserThan> :state_rootZone_moistureLevel_average ;
                                  rdfs:comment """State_rootZone_moistureLevel_low - an instance of the class caso:State that represents the root zone moisture level is at the low state.

In the example of Arvalis' dataset, this RootZoneMoistureLevel property reaches this state the open upper boundary is ST_low and the close lower boundary is ST_average.""" ;
                                  rdfs:label "State Root Zone Moisture Level Low" .


###  http://www.w3id.org/def/irrig#state_rootZone_moistureLevel_saturated
:state_rootZone_moistureLevel_saturated rdf:type owl:NamedIndividual ,
                                                 :RootZoneMoistureLevelState ;
                                        <http://www.w3id.org/def/caso#greaterThan> :state_rootZone_moistureLevel_veryHigh ;
                                        rdfs:comment """State_rootZone_moistureLevel_saturated - an instance of the class caso:State that represents the root zone moisture level is at the saturated state.

In the example of Arvalis' dataset, this RootZoneMoistureLevel property reaches this state the open upper boundary is ST_saturated and the close lower boundary is ST_minimum.""" ;
                                        rdfs:label "State Root Zone Moisture Level Saturated" .


###  http://www.w3id.org/def/irrig#state_rootZone_moistureLevel_veryHigh
:state_rootZone_moistureLevel_veryHigh rdf:type owl:NamedIndividual ,
                                                :RootZoneMoistureLevelState ;
                                       <http://www.w3id.org/def/caso#greaterThan> :state_rootZone_moistureLevel_high ;
                                       <http://www.w3id.org/def/caso#lesserThan> :state_rootZone_moistureLevel_saturated ;
                                       rdfs:comment """State_rootZone_moistureLevel_veryHigh - an instance of the class caso:State that represents the root zone moisture level is at the very high state.

In the example of Arvalis' dataset, this RootZoneMoistureLevel property reaches this state the open upper boundary is ST_very_high and the close lower boundary is ST_saturated.""" ;
                                       rdfs:label "State Root Zone Moisture Level Very High" .


###  http://www.w3id.org/def/irrig#state_rootZone_moistureLevel_veryLow
:state_rootZone_moistureLevel_veryLow rdf:type owl:NamedIndividual ,
                                               :RootZoneMoistureLevelState ;
                                      <http://www.w3id.org/def/caso#greaterThan> :state_rootZone_moistureLevel_dry ;
                                      <http://www.w3id.org/def/caso#lesserThan> :state_rootZone_moistureLevel_low ;
                                      rdfs:comment """State_rootZone_moistureLevel_veryLow - an instance of the class caso:State that represents the root zone moisture level is at the very low state.

In the example of Arvalis' dataset, this RootZoneMoistureLevel property reaches this state the open upper boundary is ST_very_low and the close lower boundary is ST_low.""" ;
                                      rdfs:label "State Root Zone Moisture Level Very Low" .


###  Generated by the OWL API (version 5.1.14) https://github.com/owlcs/owlapi/
