<?xml version="1.0"?>
<rdf:RDF xmlns="http://www.ontology.irstea.fr/irrig/"
     xml:base="http://www.ontology.irstea.fr/irrig/"
     xmlns:schema="http://schema.org/"
     xmlns:owl="http://www.w3.org/2002/07/owl#"
     xmlns:saref="https://w3id.org/saref#"
     xmlns:xsd="http://www.w3.org/2001/XMLSchema#"
     xmlns:skos="http://www.w3.org/2004/02/skos/core#"
     xmlns:rdfs="http://www.w3.org/2000/01/rdf-schema#"
     xmlns:ssn="http://www.w3.org/ns/ssn/"
     xmlns:saref4agri="https://w3id.org/def/saref4agri#"
     xmlns:rdf="http://www.w3.org/1999/02/22-rdf-syntax-ns#"
     xmlns:terms="http://purl.org/dc/terms/"
     xmlns:casoo="http://www.ontology.irstea.fr/casoo#"
     xmlns:xml="http://www.w3.org/XML/1998/namespace"
     xmlns:irrig="http://www.ontology.irstea.fr/irrig#"
     xmlns:time="http://www.w3.org/2006/time#"
     xmlns:vann="http://purl.org/vocab/vann/"
     xmlns:prov="http://www.w3.org/ns/prov#"
     xmlns:om="http://www.ontology-of-units-of-measure.org/resource/om-2/"
     xmlns:dc="http://purl.org/dc/elements/1.1/"
     xmlns:sosa="http://www.w3.org/ns/sosa/">
    <owl:Ontology rdf:about="http://www.ontology.irstea.fr/irrig/">
        <owl:versionIRI rdf:resource="http://www.ontology.irstea.fr/irrig/1.0/"/>
        <terms:creator rdf:resource="http://purl.org/net/mpoveda"/>
        <dc:title xml:lang="en">Irrigation Ontology for experimentation in TSCF, Irstea Clermont-Fd.</dc:title>
        <vann:preferredNamespaceUri>https://w3id.org/def/irrig#</vann:preferredNamespaceUri>
        <owl:versionInfo>1.0.0</owl:versionInfo>
        <terms:contributor rdf:resource="http://orcid.org/0000-0002-7011-4535"/>
        <terms:license rdf:resource="http://purl.org/NET/rdflicense/cc-by4.0"/>
        <terms:creator rdf:resource="https://orcid.org/0000-0002-3517-0945"/>
        <vann:preferredNamespacePrefix>casoo</vann:preferredNamespacePrefix>
        <rdfs:comment xml:lang="en">IRRIG is an Irrigation Ontology for experimentation in TSCF, Irstea Clermont-Fd.</rdfs:comment>
        <terms:creator rdf:resource="https://orcid.org/0000-0002-3076-5499"/>
        <dc:publisher rdf:resource="https://www.irstea.fr/en/research/research-units/tscf"/>
    </owl:Ontology>
    


    <!-- 
    ///////////////////////////////////////////////////////////////////////////////////////
    //
    // Annotation properties
    //
    ///////////////////////////////////////////////////////////////////////////////////////
     -->

    


    <!-- http://schema.org/domainIncludes -->

    <owl:AnnotationProperty rdf:about="http://schema.org/domainIncludes"/>
    


    <!-- http://schema.org/rangeIncludes -->

    <owl:AnnotationProperty rdf:about="http://schema.org/rangeIncludes"/>
    


    <!-- http://www.w3.org/2004/02/skos/core#definition -->

    <owl:AnnotationProperty rdf:about="http://www.w3.org/2004/02/skos/core#definition"/>
    


    <!-- http://www.w3.org/2004/02/skos/core#example -->

    <owl:AnnotationProperty rdf:about="http://www.w3.org/2004/02/skos/core#example"/>
    


    <!-- http://www.w3.org/2004/02/skos/core#note -->

    <owl:AnnotationProperty rdf:about="http://www.w3.org/2004/02/skos/core#note"/>
    


    <!-- 
    ///////////////////////////////////////////////////////////////////////////////////////
    //
    // Object Properties
    //
    ///////////////////////////////////////////////////////////////////////////////////////
     -->

    


    <!-- http://www.w3.org/ns/sosa/actsOnProperty -->

    <owl:ObjectProperty rdf:about="http://www.w3.org/ns/sosa/actsOnProperty">
        <owl:inverseOf rdf:resource="http://www.w3.org/ns/sosa/isActedOnBy"/>
        <rdfs:domain rdf:resource="http://www.w3.org/ns/sosa/Actuation"/>
        <rdfs:range rdf:resource="http://www.w3.org/ns/sosa/ActuatableProperty"/>
        <rdfs:comment xml:lang="en">Relation between an Actuation and the property of a FeatureOfInterest it is acting upon.</rdfs:comment>
        <rdfs:isDefinedBy rdf:resource="http://www.w3.org/ns/sosa/"/>
        <rdfs:label xml:lang="en">acts on property</rdfs:label>
        <skos:definition xml:lang="en">Relation between an Actuation and the property of a FeatureOfInterest it is acting upon.</skos:definition>
        <skos:example xml:lang="en">In the activity (Actuation) of automatically closing a window if the temperature in a room drops below 20 degrees Celsius, the property on which the Actuator acts upon is the state of the window as it changes from being open to being closed. </skos:example>
    </owl:ObjectProperty>
    


    <!-- http://www.w3.org/ns/sosa/hasFeatureOfInterest -->

    <owl:ObjectProperty rdf:about="http://www.w3.org/ns/sosa/hasFeatureOfInterest">
        <owl:inverseOf rdf:resource="http://www.w3.org/ns/sosa/isFeatureOfInterestOf"/>
        <rdfs:domain rdf:resource="http://www.w3.org/ns/sosa/Actuation"/>
        <rdfs:domain rdf:resource="http://www.w3.org/ns/sosa/Observation"/>
        <rdfs:range rdf:resource="http://www.w3.org/ns/sosa/FeatureOfInterest"/>
        <rdfs:comment xml:lang="en">A relation between an Observation and the entity whose quality was observed, or between an Actuation and the entity whose property was modified, or between an act of Sampling and the entity that was sampled.</rdfs:comment>
        <rdfs:isDefinedBy rdf:resource="http://www.w3.org/ns/sosa/"/>
        <rdfs:label xml:lang="en">has feature of interest</rdfs:label>
        <skos:definition xml:lang="en">A relation between an Observation and the entity whose quality was observed, or between an Actuation and the entity whose property was modified, or between an act of Sampling and the entity that was sampled.</skos:definition>
        <skos:example xml:lang="en">For example, in an Observation of the weight of a person, the FeatureOfInterest is the person and the property is its weight.</skos:example>
    </owl:ObjectProperty>
    


    <!-- http://www.w3.org/ns/sosa/hasResult -->

    <owl:ObjectProperty rdf:about="http://www.w3.org/ns/sosa/hasResult">
        <owl:inverseOf rdf:resource="http://www.w3.org/ns/sosa/isResultOf"/>
        <rdfs:domain rdf:resource="http://www.w3.org/ns/sosa/Actuation"/>
        <rdfs:domain rdf:resource="http://www.w3.org/ns/sosa/Observation"/>
        <rdfs:range rdf:resource="http://www.w3.org/ns/sosa/Result"/>
        <rdfs:comment xml:lang="en">Relation linking an Observation and a Sensor or Actuator and a Result, which contains a value representing the value associated with the observed Property.</rdfs:comment>
        <rdfs:comment xml:lang="en">Relation linking an Observation or Actuation or act of Sampling and a Result or Sample.</rdfs:comment>
        <rdfs:comment xml:lang="en">has result</rdfs:comment>
        <rdfs:isDefinedBy rdf:resource="http://www.w3.org/ns/sosa/"/>
        <rdfs:label xml:lang="en">has result</rdfs:label>
        <skos:definition xml:lang="en">Relation linking an Observation or Actuation or act of Sampling and a Result or Sample.</skos:definition>
    </owl:ObjectProperty>
    


    <!-- http://www.w3.org/ns/sosa/isActedOnBy -->

    <owl:ObjectProperty rdf:about="http://www.w3.org/ns/sosa/isActedOnBy"/>
    


    <!-- http://www.w3.org/ns/sosa/isFeatureOfInterestOf -->

    <owl:ObjectProperty rdf:about="http://www.w3.org/ns/sosa/isFeatureOfInterestOf"/>
    


    <!-- http://www.w3.org/ns/sosa/isObservedBy -->

    <owl:ObjectProperty rdf:about="http://www.w3.org/ns/sosa/isObservedBy"/>
    


    <!-- http://www.w3.org/ns/sosa/isResultOf -->

    <owl:ObjectProperty rdf:about="http://www.w3.org/ns/sosa/isResultOf"/>
    


    <!-- http://www.w3.org/ns/sosa/isSampleOf -->

    <owl:ObjectProperty rdf:about="http://www.w3.org/ns/sosa/isSampleOf"/>
    


    <!-- http://www.w3.org/ns/sosa/madeActuation -->

    <owl:ObjectProperty rdf:about="http://www.w3.org/ns/sosa/madeActuation">
        <owl:inverseOf rdf:resource="http://www.w3.org/ns/sosa/madeByActuator"/>
    </owl:ObjectProperty>
    


    <!-- http://www.w3.org/ns/sosa/madeByActuator -->

    <owl:ObjectProperty rdf:about="http://www.w3.org/ns/sosa/madeByActuator">
        <rdfs:domain rdf:resource="http://www.w3.org/ns/sosa/Actuation"/>
        <rdfs:range rdf:resource="http://www.w3.org/ns/sosa/Actuator"/>
        <rdfs:comment xml:lang="en">Relation linking an Actuation to the Actuator that made that Actuation.</rdfs:comment>
        <rdfs:isDefinedBy rdf:resource="http://www.w3.org/ns/sosa/"/>
        <rdfs:label xml:lang="en">made by actuator</rdfs:label>
        <skos:definition xml:lang="en">Relation linking an Actuation to the Actuator that made that Actuation.</skos:definition>
    </owl:ObjectProperty>
    


    <!-- http://www.w3.org/ns/sosa/madeBySensor -->

    <owl:ObjectProperty rdf:about="http://www.w3.org/ns/sosa/madeBySensor">
        <owl:inverseOf rdf:resource="http://www.w3.org/ns/sosa/madeObservation"/>
        <rdfs:domain rdf:resource="http://www.w3.org/ns/sosa/Observation"/>
        <rdfs:range rdf:resource="http://www.w3.org/ns/sosa/Sensor"/>
        <rdfs:comment xml:lang="en">Relation between an Observation and the Sensor which made the Observation.</rdfs:comment>
        <rdfs:isDefinedBy rdf:resource="http://www.w3.org/ns/sosa/"/>
        <rdfs:label xml:lang="en">made by sensor</rdfs:label>
        <skos:definition xml:lang="en">Relation between an Observation and the Sensor which made the Observation.</skos:definition>
    </owl:ObjectProperty>
    


    <!-- http://www.w3.org/ns/sosa/madeObservation -->

    <owl:ObjectProperty rdf:about="http://www.w3.org/ns/sosa/madeObservation"/>
    


    <!-- http://www.w3.org/ns/sosa/observedProperty -->

    <owl:ObjectProperty rdf:about="http://www.w3.org/ns/sosa/observedProperty">
        <rdfs:domain rdf:resource="http://www.w3.org/ns/sosa/Observation"/>
        <rdfs:range rdf:resource="http://www.w3.org/ns/sosa/ObservableProperty"/>
        <rdfs:comment xml:lang="en">Relation linking an Observation to the property that was observed. The ObservableProperty should be a property of the FeatureOfInterest (linked by hasFeatureOfInterest) of this Observation.</rdfs:comment>
        <rdfs:isDefinedBy rdf:resource="http://www.w3.org/ns/sosa/"/>
        <rdfs:label xml:lang="en">observed property</rdfs:label>
        <skos:definition xml:lang="en">Relation linking an Observation to the property that was observed. The ObservableProperty should be a property of the FeatureOfInterest (linked by hasFeatureOfInterest) of this Observation.</skos:definition>
    </owl:ObjectProperty>
    


    <!-- http://www.w3.org/ns/sosa/observes -->

    <owl:ObjectProperty rdf:about="http://www.w3.org/ns/sosa/observes"/>
    


    <!-- http://www.w3.org/ns/sosa/phenomenonTime -->

    <owl:ObjectProperty rdf:about="http://www.w3.org/ns/sosa/phenomenonTime">
        <rdfs:domain rdf:resource="http://www.w3.org/ns/sosa/Actuation"/>
        <rdfs:domain rdf:resource="http://www.w3.org/ns/sosa/Observation"/>
        <rdfs:range rdf:resource="http://www.w3.org/2006/time#TemporalEntity"/>
        <rdfs:comment xml:lang="en">The time that the Result of an Observation, Actuation or Sampling applies to the FeatureOfInterest. Not necessarily the same as the resultTime. May be an Interval or an Instant, or some other compound TemporalEntity.</rdfs:comment>
        <rdfs:isDefinedBy rdf:resource="http://www.w3.org/ns/sosa/"/>
        <rdfs:label xml:lang="en">phenomenon time</rdfs:label>
        <skos:definition xml:lang="en">The time that the Result of an Observation, Actuation or Sampling applies to the FeatureOfInterest. Not necessarily the same as the resultTime. May be an Interval or an Instant, or some other compound TemporalEntity.</skos:definition>
    </owl:ObjectProperty>
    


    <!-- http://www.w3.org/ns/ssn/forProperty -->

    <owl:ObjectProperty rdf:about="http://www.w3.org/ns/ssn/forProperty">
        <rdfs:domain rdf:resource="http://www.w3.org/ns/sosa/Actuator"/>
        <rdfs:range rdf:resource="http://www.w3.org/ns/sosa/ActuatableProperty"/>
        <rdfs:comment xml:lang="en">A relation between some aspect of an entity and a Property.</rdfs:comment>
        <rdfs:isDefinedBy rdf:resource="http://www.w3.org/ns/ssn/"/>
        <rdfs:label xml:lang="en">for property</rdfs:label>
        <skos:definition xml:lang="en">A relation between some aspect of an entity and a Property.</skos:definition>
        <skos:example xml:lang="en">For example, from a Sensor to the properties it can observe; from an Actuator to the properties it can act on; from a Deployment to the properties it was installed to observe or act on; from a SystemCapability to the Property the capability is described for.</skos:example>
    </owl:ObjectProperty>
    


    <!-- http://www.w3.org/ns/ssn/hasProperty -->

    <owl:ObjectProperty rdf:about="http://www.w3.org/ns/ssn/hasProperty">
        <owl:inverseOf rdf:resource="http://www.w3.org/ns/ssn/isPropertyOf"/>
        <rdfs:domain rdf:resource="http://www.w3.org/ns/sosa/FeatureOfInterest"/>
        <rdfs:range rdf:resource="http://www.w3.org/ns/ssn/Property"/>
        <rdfs:comment xml:lang="en">Relation between an entity and a Property of that entity.</rdfs:comment>
        <rdfs:isDefinedBy rdf:resource="http://www.w3.org/ns/ssn/"/>
        <rdfs:label xml:lang="en">has property</rdfs:label>
        <skos:definition xml:lang="en">Relation between an entity and a Property of that entity.</skos:definition>
    </owl:ObjectProperty>
    


    <!-- http://www.w3.org/ns/ssn/implements -->

    <owl:ObjectProperty rdf:about="http://www.w3.org/ns/ssn/implements"/>
    


    <!-- http://www.w3.org/ns/ssn/isPropertyOf -->

    <owl:ObjectProperty rdf:about="http://www.w3.org/ns/ssn/isPropertyOf"/>
    


    <!-- http://www.w3.org/ns/ssn/wasOriginatedBy -->

    <owl:ObjectProperty rdf:about="http://www.w3.org/ns/ssn/wasOriginatedBy"/>
    


    <!-- https://w3id.org/saref#hasCommand -->

    <owl:ObjectProperty rdf:about="https://w3id.org/saref#hasCommand">
        <owl:inverseOf rdf:resource="https://w3id.org/saref#isCommandOf"/>
        <rdfs:domain rdf:resource="https://w3id.org/saref#Function"/>
        <rdfs:range rdf:resource="https://w3id.org/saref#Command"/>
        <rdfs:comment>A relationship between an entity (such as a function) and a command</rdfs:comment>
        <rdfs:isDefinedBy rdf:resource="https://w3id.org/saref#"/>
        <rdfs:label>has command</rdfs:label>
    </owl:ObjectProperty>
    


    <!-- https://w3id.org/saref#isCommandOf -->

    <owl:ObjectProperty rdf:about="https://w3id.org/saref#isCommandOf">
        <rdfs:comment>A relationship between a command and a function.</rdfs:comment>
        <rdfs:isDefinedBy rdf:resource="https://w3id.org/saref#"/>
        <rdfs:label>is command of</rdfs:label>
    </owl:ObjectProperty>
    


    <!-- 
    ///////////////////////////////////////////////////////////////////////////////////////
    //
    // Data properties
    //
    ///////////////////////////////////////////////////////////////////////////////////////
     -->

    


    <!-- http://www.w3.org/ns/sosa/resultTime -->

    <owl:DatatypeProperty rdf:about="http://www.w3.org/ns/sosa/resultTime"/>
    


    <!-- https://w3id.org/saref#hasDescription -->

    <owl:DatatypeProperty rdf:about="https://w3id.org/saref#hasDescription"/>
    


    <!-- 
    ///////////////////////////////////////////////////////////////////////////////////////
    //
    // Classes
    //
    ///////////////////////////////////////////////////////////////////////////////////////
     -->

    


    <!-- http://www.ontology-of-units-of-measure.org/resource/om-2/Unit -->

    <owl:Class rdf:about="http://www.ontology-of-units-of-measure.org/resource/om-2/Unit">
        <rdfs:comment xml:lang="en">A unit of measure is a definite magnitude of a quantity, defined and adopted by convention or by law. It is used as a standard for measurement of the same quantity, where any other value of the quantity can be expressed as a simple multiple of the unit. For example, length is a quantity; the metre is a unit of length that represents a definite predetermined length. When we say 10 metre (or 10 m), we actually mean 10 times the definite predetermined length called &quot;metre&quot;.</rdfs:comment>
        <rdfs:label xml:lang="en">unit</rdfs:label>
    </owl:Class>
    


    <!-- http://www.ontology.irstea.fr/casoo#Actuation -->

    <owl:Class rdf:about="http://www.ontology.irstea.fr/casoo#Actuation">
        <rdfs:subClassOf rdf:resource="http://www.w3.org/ns/sosa/Actuation"/>
        <rdfs:comment xml:lang="en">Actuation is an action that a machine or device operate.</rdfs:comment>
        <rdfs:label xml:lang="en">Actuation</rdfs:label>
    </owl:Class>
    


    <!-- http://www.ontology.irstea.fr/casoo#Boundary -->

    <owl:Class rdf:about="http://www.ontology.irstea.fr/casoo#Boundary">
        <rdfs:comment xml:lang="en">Boundary is the limits that the State can be defined when satisfy such limits.</rdfs:comment>
        <rdfs:label xml:lang="en">Boundary</rdfs:label>
    </owl:Class>
    


    <!-- http://www.ontology.irstea.fr/casoo#Deduction -->

    <owl:Class rdf:about="http://www.ontology.irstea.fr/casoo#Deduction">
        <rdfs:subClassOf rdf:resource="http://www.ontology.irstea.fr/casoo#Observation"/>
        <rdfs:comment xml:lang="en">The result of an inference that links together a property, a state of the property and a specific time period.</rdfs:comment>
        <rdfs:label xml:lang="en">Deduction</rdfs:label>
    </owl:Class>
    


    <!-- http://www.ontology.irstea.fr/casoo#Observation -->

    <owl:Class rdf:about="http://www.ontology.irstea.fr/casoo#Observation">
        <rdfs:subClassOf rdf:resource="http://www.w3.org/ns/sosa/Observation"/>
        <rdfs:comment xml:lang="en">Observation is the action of observing or considering something.</rdfs:comment>
        <rdfs:label xml:lang="en">Observation</rdfs:label>
    </owl:Class>
    


    <!-- http://www.ontology.irstea.fr/casoo#Property -->

    <owl:Class rdf:about="http://www.ontology.irstea.fr/casoo#Property">
        <rdfs:subClassOf rdf:resource="http://www.w3.org/ns/ssn/Property"/>
        <rdfs:comment xml:lang="en">Property is an atrribute of a thing that can be used to characterize the thing.</rdfs:comment>
        <rdfs:label xml:lang="en">Property</rdfs:label>
    </owl:Class>
    


    <!-- http://www.ontology.irstea.fr/casoo#State -->

    <owl:Class rdf:about="http://www.ontology.irstea.fr/casoo#State">
        <rdfs:subClassOf rdf:resource="http://www.w3.org/2004/02/skos/core#Concept"/>
        <rdfs:comment xml:lang="en">A qualitative data which changes over time, summarizing a set of information.</rdfs:comment>
        <rdfs:label xml:lang="en">State</rdfs:label>
    </owl:Class>
    


    <!-- http://www.ontology.irstea.fr/irrig#CropGrowthBoundary -->

    <owl:Class rdf:about="http://www.ontology.irstea.fr/irrig#CropGrowthBoundary">
        <rdfs:subClassOf rdf:resource="http://www.ontology.irstea.fr/casoo#Boundary"/>
        <rdfs:comment xml:lang="en">Limits to define a crop growth state and distinguish this state to other states.</rdfs:comment>
        <rdfs:label xml:lang="en">Crop Growth Boundary</rdfs:label>
    </owl:Class>
    


    <!-- http://www.ontology.irstea.fr/irrig#CropGrowthDeduction -->

    <owl:Class rdf:about="http://www.ontology.irstea.fr/irrig#CropGrowthDeduction">
        <rdfs:subClassOf rdf:resource="http://www.ontology.irstea.fr/casoo#Deduction"/>
        <rdfs:comment xml:lang="en">The inference result that determine the crop growth state at a specific time.</rdfs:comment>
        <rdfs:label xml:lang="en">Crop Growth Deduction</rdfs:label>
    </owl:Class>
    


    <!-- http://www.ontology.irstea.fr/irrig#CropGrowthObservation -->

    <owl:Class rdf:about="http://www.ontology.irstea.fr/irrig#CropGrowthObservation">
        <rdfs:subClassOf rdf:resource="http://www.ontology.irstea.fr/casoo#Observation"/>
        <rdfs:comment xml:lang="en">The act that a sensor carries out an crop growth observation.</rdfs:comment>
        <rdfs:label xml:lang="en">Crop growth observation</rdfs:label>
    </owl:Class>
    


    <!-- http://www.ontology.irstea.fr/irrig#CropGrowthState -->

    <owl:Class rdf:about="http://www.ontology.irstea.fr/irrig#CropGrowthState">
        <rdfs:subClassOf rdf:resource="http://www.ontology.irstea.fr/casoo#State"/>
        <rdfs:comment xml:lang="en">Situation that a crop growth property has qualitative data that distinguish with other situations. This is a definitive class including the following states: init, v2, v7, v7d25, r1, r1d15, r5, r5hg45.</rdfs:comment>
        <rdfs:label xml:lang="en">Crop Growth State</rdfs:label>
    </owl:Class>
    


    <!-- http://www.ontology.irstea.fr/irrig#CropWaterNeedBoundary -->

    <owl:Class rdf:about="http://www.ontology.irstea.fr/irrig#CropWaterNeedBoundary">
        <rdfs:subClassOf rdf:resource="http://www.ontology.irstea.fr/casoo#Boundary"/>
        <rdfs:comment xml:lang="en">Limits to define a crop water need state and distinguish this state to other states.</rdfs:comment>
    </owl:Class>
    


    <!-- http://www.ontology.irstea.fr/irrig#CropWaterNeedDeduction -->

    <owl:Class rdf:about="http://www.ontology.irstea.fr/irrig#CropWaterNeedDeduction">
        <rdfs:subClassOf rdf:resource="http://www.ontology.irstea.fr/casoo#Deduction"/>
        <rdfs:comment xml:lang="en">The inference result that determine the crop water need state at a specific time.</rdfs:comment>
        <rdfs:label xml:lang="en">Crop Water Need Deduction</rdfs:label>
    </owl:Class>
    


    <!-- http://www.ontology.irstea.fr/irrig#CropWaterNeedState -->

    <owl:Class rdf:about="http://www.ontology.irstea.fr/irrig#CropWaterNeedState">
        <rdfs:subClassOf rdf:resource="http://www.ontology.irstea.fr/casoo#State"/>
        <rdfs:comment xml:lang="en">Situation that a crop water need property has qualitative data that distinguish with other situations. This is a definitive class including the following states: init, no, yes, wait.</rdfs:comment>
        <rdfs:label xml:lang="en">Crop Water Need State</rdfs:label>
    </owl:Class>
    


    <!-- http://www.ontology.irstea.fr/irrig#GrowthPorperty -->

    <owl:Class rdf:about="http://www.ontology.irstea.fr/irrig#GrowthPorperty">
        <rdfs:subClassOf rdf:resource="http://www.w3.org/ns/ssn/Property"/>
        <rdfs:comment xml:lang="en">Property dedicated to the growth of plants.</rdfs:comment>
        <rdfs:label xml:lang="en">Growth property</rdfs:label>
    </owl:Class>
    


    <!-- http://www.ontology.irstea.fr/irrig#IrrigationActuation -->

    <owl:Class rdf:about="http://www.ontology.irstea.fr/irrig#IrrigationActuation">
        <rdfs:subClassOf rdf:resource="http://www.ontology.irstea.fr/casoo#Actuation"/>
        <rdfs:comment xml:lang="en">The act that an actuator carries out an irrigation action.</rdfs:comment>
        <rdfs:label xml:lang="en">Irrigation actuation</rdfs:label>
    </owl:Class>
    


    <!-- http://www.ontology.irstea.fr/irrig#MoistureProperty -->

    <owl:Class rdf:about="http://www.ontology.irstea.fr/irrig#MoistureProperty">
        <rdfs:subClassOf rdf:resource="http://www.w3.org/ns/ssn/Property"/>
        <rdfs:comment xml:lang="en">Property dedicated to the moisture in the soil.</rdfs:comment>
        <rdfs:label xml:lang="en">Moisture property</rdfs:label>
    </owl:Class>
    


    <!-- http://www.ontology.irstea.fr/irrig#RootZoneMoistureLevelBoundary -->

    <owl:Class rdf:about="http://www.ontology.irstea.fr/irrig#RootZoneMoistureLevelBoundary">
        <rdfs:subClassOf rdf:resource="http://www.ontology.irstea.fr/casoo#Boundary"/>
        <rdfs:comment xml:lang="en">Limits to define a root zone moisture level state and distinguish this state to other states.</rdfs:comment>
        <rdfs:label xml:lang="en">Root Zone Moisture Level Boundary</rdfs:label>
    </owl:Class>
    


    <!-- http://www.ontology.irstea.fr/irrig#RootZoneMoistureLevelDeduction -->

    <owl:Class rdf:about="http://www.ontology.irstea.fr/irrig#RootZoneMoistureLevelDeduction">
        <rdfs:subClassOf rdf:resource="http://www.ontology.irstea.fr/casoo#Deduction"/>
        <rdfs:comment xml:lang="en">The inference result that determine the rootzone moisture level state at a specific time.</rdfs:comment>
        <rdfs:label xml:lang="en">Root Zone Moisture Level Deduction</rdfs:label>
    </owl:Class>
    


    <!-- http://www.ontology.irstea.fr/irrig#RootZoneMoistureLevelState -->

    <owl:Class rdf:about="http://www.ontology.irstea.fr/irrig#RootZoneMoistureLevelState">
        <rdfs:subClassOf rdf:resource="http://www.ontology.irstea.fr/casoo#State"/>
        <rdfs:comment xml:lang="en">Situation that a root zone moisture level has qualitative data that distinguish with other situation. This is a definitive class including the following states: init, saturated, very high, high, average, low, very low, dry.</rdfs:comment>
        <rdfs:label xml:lang="en">Root Zone Moisture Level State</rdfs:label>
    </owl:Class>
    


    <!-- http://www.ontology.irstea.fr/irrig#RootZoneMoisturePerDayObservation -->

    <owl:Class rdf:about="http://www.ontology.irstea.fr/irrig#RootZoneMoisturePerDayObservation">
        <rdfs:subClassOf rdf:resource="http://www.ontology.irstea.fr/casoo#Observation"/>
        <rdfs:comment xml:lang="en">The act that a sensor carries out an root zone moisture per day observation.</rdfs:comment>
        <rdfs:label xml:lang="en">Root zone moisture per day observation</rdfs:label>
    </owl:Class>
    


    <!-- http://www.ontology.irstea.fr/irrig#Soil30cmDepthAverageMoisturePerDayObservation -->

    <owl:Class rdf:about="http://www.ontology.irstea.fr/irrig#Soil30cmDepthAverageMoisturePerDayObservation">
        <rdfs:subClassOf rdf:resource="http://www.ontology.irstea.fr/casoo#Observation"/>
        <rdfs:comment xml:lang="en">The act that a sensor carries out an average moisture per day observation at 30 cmp depth soil.</rdfs:comment>
        <rdfs:label xml:lang="en">Soil 30cm Depth Average Moisture Per Day Observation</rdfs:label>
    </owl:Class>
    


    <!-- http://www.ontology.irstea.fr/irrig#Soil30cmDepthMoistureObservation -->

    <owl:Class rdf:about="http://www.ontology.irstea.fr/irrig#Soil30cmDepthMoistureObservation">
        <rdfs:subClassOf rdf:resource="http://www.ontology.irstea.fr/casoo#Observation"/>
        <rdfs:comment xml:lang="en">The act that a sensor carries out a moisture observation at 30 cm depth soil.</rdfs:comment>
        <rdfs:label xml:lang="en">Soil 30cm Depth Moisture Observation</rdfs:label>
    </owl:Class>
    


    <!-- http://www.ontology.irstea.fr/irrig#Soil60cmDepthAverageMoisturePerDayObservation -->

    <owl:Class rdf:about="http://www.ontology.irstea.fr/irrig#Soil60cmDepthAverageMoisturePerDayObservation">
        <rdfs:subClassOf rdf:resource="http://www.ontology.irstea.fr/casoo#Observation"/>
        <rdfs:comment xml:lang="en">The act that a sensor carries out an average moisture per day observation at 60 cmp depth soil.</rdfs:comment>
        <rdfs:label xml:lang="en">Soil 60cm Depth Average Moisture Per Day Observation</rdfs:label>
    </owl:Class>
    


    <!-- http://www.ontology.irstea.fr/irrig#Soil60cmDepthMoistureObservation -->

    <owl:Class rdf:about="http://www.ontology.irstea.fr/irrig#Soil60cmDepthMoistureObservation">
        <rdfs:subClassOf rdf:resource="http://www.ontology.irstea.fr/casoo#Observation"/>
        <rdfs:comment xml:lang="en">The act that a sensor carries out a moisture observation at 60 cm depth soil.</rdfs:comment>
        <rdfs:label xml:lang="en">Soil 60cm Depth Moisture Observation</rdfs:label>
    </owl:Class>
    


    <!-- http://www.ontology.irstea.fr/irrig#StressProperty -->

    <owl:Class rdf:about="http://www.ontology.irstea.fr/irrig#StressProperty">
        <rdfs:subClassOf rdf:resource="http://www.w3.org/ns/ssn/Property"/>
        <rdfs:comment xml:lang="en">Property dedicated to the stress of plants.</rdfs:comment>
        <rdfs:label xml:lang="en">Stress property</rdfs:label>
    </owl:Class>
    


    <!-- http://www.ontology.irstea.fr/irrig#Unit -->

    <owl:Class rdf:about="http://www.ontology.irstea.fr/irrig#Unit">
        <rdfs:comment xml:lang="en">Unit for irrigation and agriculture domain.</rdfs:comment>
        <rdfs:label xml:lang="en">Unit</rdfs:label>
    </owl:Class>
    


    <!-- http://www.w3.org/2004/02/skos/core#Concept -->

    <owl:Class rdf:about="http://www.w3.org/2004/02/skos/core#Concept">
        <rdfs:comment xml:lang="en">The class skos:Concept is the class of SKOS concepts.

A SKOS concept can be viewed as an idea or notion; a unit of thought. However, what constitutes a unit of thought is subjective, and this definition is meant to be suggestive, rather than restrictive.

The notion of a SKOS concept is useful when describing the conceptual or intellectual structure of a knowledge organization system, and when referring to specific ideas or meanings established within a KOS.

Note that, because SKOS is designed to be a vehicle for representing semi-formal KOS, such as thesauri and classification schemes, a certain amount of flexibility has been built in to the formal definition of this class.</rdfs:comment>
        <rdfs:label xml:lang="en">Concept</rdfs:label>
    </owl:Class>
    


    <!-- http://www.w3.org/2006/time#TemporalEntity -->

    <owl:Class rdf:about="http://www.w3.org/2006/time#TemporalEntity">
        <rdfs:isDefinedBy>http://www.w3.org/2006/time#</rdfs:isDefinedBy>
        <rdfs:label xml:lang="en">Temporal entity</rdfs:label>
    </owl:Class>
    


    <!-- http://www.w3.org/ns/sosa/ActuatableProperty -->

    <owl:Class rdf:about="http://www.w3.org/ns/sosa/ActuatableProperty">
        <rdfs:subClassOf rdf:resource="http://www.w3.org/ns/ssn/Property"/>
        <rdfs:subClassOf>
            <owl:Restriction>
                <owl:onProperty rdf:resource="http://www.w3.org/ns/sosa/isActedOnBy"/>
                <owl:allValuesFrom rdf:resource="http://www.w3.org/ns/sosa/Actuation"/>
            </owl:Restriction>
        </rdfs:subClassOf>
        <rdfs:comment xml:lang="en">An actuatable quality (property, characteristic) of a FeatureOfInterest.</rdfs:comment>
        <rdfs:isDefinedBy rdf:resource="http://www.w3.org/ns/sosa/"/>
        <rdfs:label xml:lang="en">Actuatable Property</rdfs:label>
        <skos:definition xml:lang="en">An actuatable quality (property, characteristic) of a FeatureOfInterest.</skos:definition>
        <skos:example xml:lang="en">A window actuator acts by changing the state between a frame and a window. The ability of the window to be opened and closed is its ActuatableProperty.</skos:example>
    </owl:Class>
    


    <!-- http://www.w3.org/ns/sosa/Actuation -->

    <owl:Class rdf:about="http://www.w3.org/ns/sosa/Actuation">
        <rdfs:subClassOf>
            <owl:Restriction>
                <owl:onProperty rdf:resource="http://www.w3.org/ns/sosa/actsOnProperty"/>
                <owl:allValuesFrom rdf:resource="http://www.w3.org/ns/sosa/ActuatableProperty"/>
            </owl:Restriction>
        </rdfs:subClassOf>
        <rdfs:subClassOf>
            <owl:Restriction>
                <owl:onProperty rdf:resource="http://www.w3.org/ns/sosa/hasFeatureOfInterest"/>
                <owl:allValuesFrom rdf:resource="http://www.w3.org/ns/sosa/FeatureOfInterest"/>
            </owl:Restriction>
        </rdfs:subClassOf>
        <rdfs:subClassOf>
            <owl:Restriction>
                <owl:onProperty rdf:resource="http://www.w3.org/ns/sosa/hasResult"/>
                <owl:allValuesFrom rdf:resource="http://www.w3.org/ns/sosa/Result"/>
            </owl:Restriction>
        </rdfs:subClassOf>
        <rdfs:subClassOf>
            <owl:Restriction>
                <owl:onProperty rdf:resource="http://www.w3.org/ns/sosa/madeByActuator"/>
                <owl:allValuesFrom rdf:resource="http://www.w3.org/ns/sosa/Actuator"/>
            </owl:Restriction>
        </rdfs:subClassOf>
        <rdfs:subClassOf>
            <owl:Restriction>
                <owl:onProperty rdf:resource="http://www.w3.org/ns/sosa/actsOnProperty"/>
                <owl:minCardinality rdf:datatype="http://www.w3.org/2001/XMLSchema#nonNegativeInteger">1</owl:minCardinality>
            </owl:Restriction>
        </rdfs:subClassOf>
        <rdfs:subClassOf>
            <owl:Restriction>
                <owl:onProperty rdf:resource="http://www.w3.org/ns/sosa/hasResult"/>
                <owl:minCardinality rdf:datatype="http://www.w3.org/2001/XMLSchema#nonNegativeInteger">1</owl:minCardinality>
            </owl:Restriction>
        </rdfs:subClassOf>
        <rdfs:subClassOf>
            <owl:Restriction>
                <owl:onProperty rdf:resource="http://www.w3.org/ns/sosa/hasFeatureOfInterest"/>
                <owl:cardinality rdf:datatype="http://www.w3.org/2001/XMLSchema#nonNegativeInteger">1</owl:cardinality>
            </owl:Restriction>
        </rdfs:subClassOf>
        <rdfs:subClassOf>
            <owl:Restriction>
                <owl:onProperty rdf:resource="http://www.w3.org/ns/sosa/madeByActuator"/>
                <owl:cardinality rdf:datatype="http://www.w3.org/2001/XMLSchema#nonNegativeInteger">1</owl:cardinality>
            </owl:Restriction>
        </rdfs:subClassOf>
        <rdfs:subClassOf>
            <owl:Restriction>
                <owl:onProperty rdf:resource="http://www.w3.org/ns/sosa/resultTime"/>
                <owl:cardinality rdf:datatype="http://www.w3.org/2001/XMLSchema#nonNegativeInteger">1</owl:cardinality>
            </owl:Restriction>
        </rdfs:subClassOf>
        <rdfs:comment xml:lang="en">An Actuation carries out an (Actuation) Procedure to change the state of the world using an Actuator.</rdfs:comment>
        <rdfs:isDefinedBy rdf:resource="http://www.w3.org/ns/sosa/"/>
        <rdfs:label xml:lang="en">Actuation</rdfs:label>
        <skos:definition xml:lang="en">An Actuation carries out an (Actuation) Procedure to change the state of the world using an Actuator.</skos:definition>
        <skos:example xml:lang="en">The activity of automatically closing a window if the temperature in a room drops below 20 degree Celsius. The activity is the Actuation and the device that closes the window is the Actuator. The Procedure is the rule, plan, or specification that defines the conditions that triggers the Actuation, here a drop in temperature. </skos:example>
    </owl:Class>
    


    <!-- http://www.w3.org/ns/sosa/Actuator -->

    <owl:Class rdf:about="http://www.w3.org/ns/sosa/Actuator">
        <rdfs:subClassOf rdf:resource="http://www.w3.org/ns/ssn/System"/>
        <rdfs:subClassOf>
            <owl:Restriction>
                <owl:onProperty rdf:resource="http://www.w3.org/ns/sosa/madeActuation"/>
                <owl:allValuesFrom rdf:resource="http://www.w3.org/ns/sosa/Actuation"/>
            </owl:Restriction>
        </rdfs:subClassOf>
        <rdfs:subClassOf>
            <owl:Restriction>
                <owl:onProperty rdf:resource="http://www.w3.org/ns/ssn/forProperty"/>
                <owl:allValuesFrom rdf:resource="http://www.w3.org/ns/sosa/ActuatableProperty"/>
            </owl:Restriction>
        </rdfs:subClassOf>
        <rdfs:subClassOf>
            <owl:Restriction>
                <owl:onProperty rdf:resource="http://www.w3.org/ns/ssn/implements"/>
                <owl:minCardinality rdf:datatype="http://www.w3.org/2001/XMLSchema#nonNegativeInteger">1</owl:minCardinality>
            </owl:Restriction>
        </rdfs:subClassOf>
        <rdfs:comment xml:lang="en">A device that is used by, or implements, an (Actuation) Procedure that changes the state of the world.</rdfs:comment>
        <rdfs:isDefinedBy rdf:resource="http://www.w3.org/ns/sosa/"/>
        <rdfs:label xml:lang="en">Actuator</rdfs:label>
        <skos:definition xml:lang="en">A device that is used by, or implements, an (Actuation) Procedure that changes the state of the world.</skos:definition>
        <skos:example xml:lang="en">A window actuator for automatic window control, i.e., opening or closing the window.</skos:example>
    </owl:Class>
    


    <!-- http://www.w3.org/ns/sosa/FeatureOfInterest -->

    <owl:Class rdf:about="http://www.w3.org/ns/sosa/FeatureOfInterest">
        <rdfs:subClassOf>
            <owl:Restriction>
                <owl:onProperty rdf:resource="http://www.w3.org/ns/ssn/hasProperty"/>
                <owl:allValuesFrom rdf:resource="http://www.w3.org/ns/ssn/Property"/>
            </owl:Restriction>
        </rdfs:subClassOf>
        <rdfs:subClassOf>
            <owl:Restriction>
                <owl:onProperty rdf:resource="http://www.w3.org/ns/ssn/hasProperty"/>
                <owl:minCardinality rdf:datatype="http://www.w3.org/2001/XMLSchema#nonNegativeInteger">1</owl:minCardinality>
            </owl:Restriction>
        </rdfs:subClassOf>
        <rdfs:comment xml:lang="en">The thing whose property is being estimated or calculated in the course of an Observation to arrive at a Result or whose property is being manipulated by an Actuator, or which is being sampled or transformed in an act of Sampling.</rdfs:comment>
        <rdfs:isDefinedBy rdf:resource="http://www.w3.org/ns/sosa/"/>
        <rdfs:label xml:lang="en">Feature Of Interest</rdfs:label>
        <skos:definition xml:lang="en">The thing whose property is being estimated or calculated in the course of an Observation to arrive at a Result or whose property is being manipulated by an Actuator, or which is being sampled or transformed in an act of Sampling.</skos:definition>
        <skos:example xml:lang="en">When measuring the height of a tree, the height is the observed ObservableProperty, 20m may be the Result of the Observation, and the tree is the FeatureOfInterest. A window is a FeatureOfInterest for an automatic window control Actuator.</skos:example>
    </owl:Class>
    


    <!-- http://www.w3.org/ns/sosa/ObservableProperty -->

    <owl:Class rdf:about="http://www.w3.org/ns/sosa/ObservableProperty">
        <rdfs:subClassOf rdf:resource="http://www.w3.org/ns/ssn/Property"/>
        <rdfs:subClassOf>
            <owl:Restriction>
                <owl:onProperty rdf:resource="http://www.w3.org/ns/sosa/isObservedBy"/>
                <owl:allValuesFrom rdf:resource="http://www.w3.org/ns/sosa/Sensor"/>
            </owl:Restriction>
        </rdfs:subClassOf>
        <rdfs:subClassOf>
            <owl:Restriction>
                <owl:onProperty>
                    <rdf:Description>
                        <owl:inverseOf rdf:resource="http://www.w3.org/ns/sosa/observedProperty"/>
                    </rdf:Description>
                </owl:onProperty>
                <owl:allValuesFrom rdf:resource="http://www.w3.org/ns/sosa/Observation"/>
            </owl:Restriction>
        </rdfs:subClassOf>
        <rdfs:comment xml:lang="en">An observable quality (property, characteristic) of a FeatureOfInterest.</rdfs:comment>
        <rdfs:isDefinedBy rdf:resource="http://www.w3.org/ns/sosa/"/>
        <rdfs:label xml:lang="en">Observable Property</rdfs:label>
        <skos:definition xml:lang="en">An observable quality (property, characteristic) of a FeatureOfInterest.</skos:definition>
        <skos:example xml:lang="en">The height of a tree, the depth of a water body, or the temperature of a surface are examples of observable properties, while the value of a classic car is not (directly) observable but asserted.</skos:example>
    </owl:Class>
    


    <!-- http://www.w3.org/ns/sosa/Observation -->

    <owl:Class rdf:about="http://www.w3.org/ns/sosa/Observation">
        <rdfs:subClassOf>
            <owl:Restriction>
                <owl:onProperty rdf:resource="http://www.w3.org/ns/sosa/hasFeatureOfInterest"/>
                <owl:allValuesFrom rdf:resource="http://www.w3.org/ns/sosa/FeatureOfInterest"/>
            </owl:Restriction>
        </rdfs:subClassOf>
        <rdfs:subClassOf>
            <owl:Restriction>
                <owl:onProperty rdf:resource="http://www.w3.org/ns/sosa/hasResult"/>
                <owl:allValuesFrom rdf:resource="http://www.w3.org/ns/sosa/Result"/>
            </owl:Restriction>
        </rdfs:subClassOf>
        <rdfs:subClassOf>
            <owl:Restriction>
                <owl:onProperty rdf:resource="http://www.w3.org/ns/sosa/madeBySensor"/>
                <owl:allValuesFrom rdf:resource="http://www.w3.org/ns/sosa/Sensor"/>
            </owl:Restriction>
        </rdfs:subClassOf>
        <rdfs:subClassOf>
            <owl:Restriction>
                <owl:onProperty rdf:resource="http://www.w3.org/ns/sosa/observedProperty"/>
                <owl:allValuesFrom rdf:resource="http://www.w3.org/ns/sosa/ObservableProperty"/>
            </owl:Restriction>
        </rdfs:subClassOf>
        <rdfs:subClassOf>
            <owl:Restriction>
                <owl:onProperty rdf:resource="http://www.w3.org/ns/sosa/hasResult"/>
                <owl:minCardinality rdf:datatype="http://www.w3.org/2001/XMLSchema#nonNegativeInteger">1</owl:minCardinality>
            </owl:Restriction>
        </rdfs:subClassOf>
        <rdfs:subClassOf>
            <owl:Restriction>
                <owl:onProperty rdf:resource="http://www.w3.org/ns/sosa/hasFeatureOfInterest"/>
                <owl:cardinality rdf:datatype="http://www.w3.org/2001/XMLSchema#nonNegativeInteger">1</owl:cardinality>
            </owl:Restriction>
        </rdfs:subClassOf>
        <rdfs:subClassOf>
            <owl:Restriction>
                <owl:onProperty rdf:resource="http://www.w3.org/ns/sosa/madeBySensor"/>
                <owl:cardinality rdf:datatype="http://www.w3.org/2001/XMLSchema#nonNegativeInteger">1</owl:cardinality>
            </owl:Restriction>
        </rdfs:subClassOf>
        <rdfs:subClassOf>
            <owl:Restriction>
                <owl:onProperty rdf:resource="http://www.w3.org/ns/sosa/observedProperty"/>
                <owl:cardinality rdf:datatype="http://www.w3.org/2001/XMLSchema#nonNegativeInteger">1</owl:cardinality>
            </owl:Restriction>
        </rdfs:subClassOf>
        <rdfs:subClassOf>
            <owl:Restriction>
                <owl:onProperty rdf:resource="http://www.w3.org/ns/sosa/phenomenonTime"/>
                <owl:cardinality rdf:datatype="http://www.w3.org/2001/XMLSchema#nonNegativeInteger">1</owl:cardinality>
            </owl:Restriction>
        </rdfs:subClassOf>
        <rdfs:subClassOf>
            <owl:Restriction>
                <owl:onProperty rdf:resource="http://www.w3.org/ns/ssn/wasOriginatedBy"/>
                <owl:cardinality rdf:datatype="http://www.w3.org/2001/XMLSchema#nonNegativeInteger">1</owl:cardinality>
            </owl:Restriction>
        </rdfs:subClassOf>
        <rdfs:subClassOf>
            <owl:Restriction>
                <owl:onProperty rdf:resource="http://www.w3.org/ns/sosa/resultTime"/>
                <owl:cardinality rdf:datatype="http://www.w3.org/2001/XMLSchema#nonNegativeInteger">1</owl:cardinality>
            </owl:Restriction>
        </rdfs:subClassOf>
        <rdfs:comment xml:lang="en">Act of carrying out an (Observation) Procedure to estimate or calculate a value of a property of a FeatureOfInterest. Links to a Sensor to describe what made the Observation and how; links to an ObservableProperty to describe what the result is an estimate of, and to a FeatureOfInterest to detail what that property was associated with.</rdfs:comment>
        <rdfs:comment xml:lang="en">Observation - Act of carrying out an (Observation) Procedure to estimate or calculate a value of a property of a FeatureOfInterest. Links to a Sensor to describe what made the Observation and how; links to an ObservableProperty to describe what the result is an estimate of, and to a FeatureOfInterest to detail what that property was associated with.</rdfs:comment>
        <rdfs:isDefinedBy rdf:resource="http://www.w3.org/ns/sosa/"/>
        <rdfs:label xml:lang="en">Observation</rdfs:label>
        <skos:definition xml:lang="en">Act of carrying out an (Observation) Procedure to estimate or calculate a value of a property of a FeatureOfInterest. Links to a Sensor to describe what made the Observation and how; links to an ObservableProperty to describe what the result is an estimate of, and to a FeatureOfInterest to detail what that property was associated with.</skos:definition>
        <skos:example xml:lang="en">The activity of estimating the intensity of an Earthquake using the Mercalli intensity scale is an Observation as is measuring the moment magnitude, i.e., the energy released by said earthquake.</skos:example>
    </owl:Class>
    


    <!-- http://www.w3.org/ns/sosa/Result -->

    <owl:Class rdf:about="http://www.w3.org/ns/sosa/Result">
        <rdfs:subClassOf>
            <owl:Restriction>
                <owl:onProperty rdf:resource="http://www.w3.org/ns/sosa/isResultOf"/>
                <owl:minCardinality rdf:datatype="http://www.w3.org/2001/XMLSchema#nonNegativeInteger">1</owl:minCardinality>
            </owl:Restriction>
        </rdfs:subClassOf>
        <rdfs:comment xml:lang="en">The Result of an Observation, Actuation, or act of Sampling. To store an observation&apos;s simple result value one can use the hasSimpleResult property.</rdfs:comment>
        <rdfs:isDefinedBy rdf:resource="http://www.w3.org/ns/sosa/"/>
        <rdfs:label xml:lang="en">Result</rdfs:label>
        <skos:definition xml:lang="en">The Result of an Observation, Actuation, or act of Sampling. To store an observation&apos;s simple result value one can use the hasSimpleResult property.</skos:definition>
        <skos:example xml:lang="en">The value 20 as the height of a certain tree together with the unit, e.g., Meter.</skos:example>
    </owl:Class>
    


    <!-- http://www.w3.org/ns/sosa/Sample -->

    <owl:Class rdf:about="http://www.w3.org/ns/sosa/Sample">
        <rdfs:subClassOf rdf:resource="http://www.w3.org/ns/sosa/FeatureOfInterest"/>
        <rdfs:subClassOf rdf:resource="http://www.w3.org/ns/sosa/Result"/>
        <rdfs:subClassOf>
            <owl:Restriction>
                <owl:onProperty rdf:resource="http://www.w3.org/ns/sosa/isResultOf"/>
                <owl:allValuesFrom rdf:resource="http://www.w3.org/ns/sosa/Sampling"/>
            </owl:Restriction>
        </rdfs:subClassOf>
        <rdfs:subClassOf>
            <owl:Restriction>
                <owl:onProperty rdf:resource="http://www.w3.org/ns/sosa/isSampleOf"/>
                <owl:allValuesFrom rdf:resource="http://www.w3.org/ns/sosa/FeatureOfInterest"/>
            </owl:Restriction>
        </rdfs:subClassOf>
        <rdfs:subClassOf>
            <owl:Restriction>
                <owl:onProperty rdf:resource="http://www.w3.org/ns/sosa/isResultOf"/>
                <owl:minCardinality rdf:datatype="http://www.w3.org/2001/XMLSchema#nonNegativeInteger">1</owl:minCardinality>
            </owl:Restriction>
        </rdfs:subClassOf>
        <rdfs:subClassOf>
            <owl:Restriction>
                <owl:onProperty rdf:resource="http://www.w3.org/ns/sosa/isSampleOf"/>
                <owl:minCardinality rdf:datatype="http://www.w3.org/2001/XMLSchema#nonNegativeInteger">1</owl:minCardinality>
            </owl:Restriction>
        </rdfs:subClassOf>
        <rdfs:comment xml:lang="en">A Sample is the result from an act of Sampling.</rdfs:comment>
        <rdfs:comment xml:lang="en">Feature which is intended to be representative of a FeatureOfInterest on which Observations may be made.</rdfs:comment>
        <rdfs:comment xml:lang="en">Physical samples are sometimes known as &apos;specimens&apos;.</rdfs:comment>
        <rdfs:comment xml:lang="en">Samples are artifacts of an observational strategy, and have no significant function outside of their role in the observation process. The characteristics of the samples themselves are of little interest, except perhaps to the manager of a sampling campaign.

A Sample is intended to sample some FatureOfInterest, so there is an expectation of at least one isSampleOf property. However, in some cases the identity, and even the exact type, of the sampled feature may not be known when observations are made using the sampling features.</rdfs:comment>
        <rdfs:isDefinedBy rdf:resource="http://www.w3.org/ns/sosa/"/>
        <rdfs:label xml:lang="en">Sample</rdfs:label>
        <skos:definition xml:lang="en">Feature which is intended to be representative of a FeatureOfInterest on which Observations may be made.</skos:definition>
        <skos:example xml:lang="en">A &apos;station&apos; is essentially an identifiable locality where a sensor system or Procedure may be deployed and an observation made. In the context of the observation model, it connotes the &apos;world in the vicinity of the station&apos;, so the observed properties relate to the physical medium at the station, and not to any physical artifact such as a mooring, buoy, benchmark, monument, well, etc.</skos:example>
        <skos:example xml:lang="en">A statistical sample is often designed to be characteristic of an entire population, so that observations can be made regarding the sample that provide a good estimate of the properties of the population.</skos:example>
        <skos:note xml:lang="en">A transient sample, such as a ships-track or flight-line, might be identified and described, but is unlikely to be revisited exactly.</skos:note>
    </owl:Class>
    


    <!-- http://www.w3.org/ns/sosa/Sampling -->

    <owl:Class rdf:about="http://www.w3.org/ns/sosa/Sampling">
        <rdfs:comment xml:lang="en">An act of Sampling carries out a (Sampling) Procedure to create or transform one or more Samples.</rdfs:comment>
        <rdfs:label xml:lang="en">Sampling</rdfs:label>
    </owl:Class>
    


    <!-- http://www.w3.org/ns/sosa/Sensor -->

    <owl:Class rdf:about="http://www.w3.org/ns/sosa/Sensor">
        <rdfs:subClassOf rdf:resource="http://www.w3.org/ns/ssn/System"/>
        <rdfs:subClassOf>
            <owl:Restriction>
                <owl:onProperty rdf:resource="http://www.w3.org/ns/sosa/madeObservation"/>
                <owl:allValuesFrom rdf:resource="http://www.w3.org/ns/sosa/Observation"/>
            </owl:Restriction>
        </rdfs:subClassOf>
        <rdfs:subClassOf>
            <owl:Restriction>
                <owl:onProperty rdf:resource="http://www.w3.org/ns/sosa/observes"/>
                <owl:allValuesFrom rdf:resource="http://www.w3.org/ns/sosa/ObservableProperty"/>
            </owl:Restriction>
        </rdfs:subClassOf>
        <rdfs:subClassOf>
            <owl:Restriction>
                <owl:onProperty rdf:resource="http://www.w3.org/ns/ssn/implements"/>
                <owl:minCardinality rdf:datatype="http://www.w3.org/2001/XMLSchema#nonNegativeInteger">1</owl:minCardinality>
            </owl:Restriction>
        </rdfs:subClassOf>
        <rdfs:comment xml:lang="en">Device, agent (including humans), or software (simulation) involved in, or implementing, a Procedure. Sensors respond to a stimulus, e.g., a change in the environment, or input data composed from the results of prior Observations, and generate a Result. Sensors can be hosted by Platforms.</rdfs:comment>
        <rdfs:isDefinedBy rdf:resource="http://www.w3.org/ns/sosa/"/>
        <rdfs:label xml:lang="en">Sensor</rdfs:label>
        <skos:definition xml:lang="en">Device, agent (including humans), or software (simulation) involved in, or implementing, a Procedure. Sensors respond to a stimulus, e.g., a change in the environment, or input data composed from the results of prior Observations, and generate a Result. Sensors can be hosted by Platforms.</skos:definition>
        <skos:example xml:lang="en">Accelerometers, gyroscopes, barometers, magnetometers, and so forth are Sensors that are typically mounted on a modern smart phone (which acts as Platform). Other examples of sensors include the human eyes.</skos:example>
    </owl:Class>
    


    <!-- http://www.w3.org/ns/ssn/Property -->

    <owl:Class rdf:about="http://www.w3.org/ns/ssn/Property">
        <rdfs:subClassOf>
            <owl:Restriction>
                <owl:onProperty rdf:resource="http://www.w3.org/ns/ssn/isPropertyOf"/>
                <owl:allValuesFrom rdf:resource="http://www.w3.org/ns/sosa/FeatureOfInterest"/>
            </owl:Restriction>
        </rdfs:subClassOf>
        <rdfs:comment xml:lang="en">A quality of an entity. An aspect of an entity that is intrinsic to and cannot exist without the entity.</rdfs:comment>
        <rdfs:isDefinedBy rdf:resource="http://www.w3.org/ns/ssn/"/>
        <rdfs:label xml:lang="en">Property</rdfs:label>
        <skos:definition xml:lang="en">A quality of an entity. An aspect of an entity that is intrinsic to and cannot exist without the entity.</skos:definition>
    </owl:Class>
    


    <!-- http://www.w3.org/ns/ssn/System -->

    <owl:Class rdf:about="http://www.w3.org/ns/ssn/System">
        <rdfs:comment xml:lang="en">System is a unit of abstraction for pieces of infrastructure that implement Procedures. A System may have components, its subsystems, which are other Systems.</rdfs:comment>
        <rdfs:label xml:lang="en">System</rdfs:label>
    </owl:Class>
    


    <!-- https://w3id.org/def/saref4agri#Pluviometer -->

    <owl:Class rdf:about="https://w3id.org/def/saref4agri#Pluviometer">
        <rdfs:subClassOf rdf:resource="https://w3id.org/saref#Sensor"/>
        <rdfs:label xml:lang="en">A sensor that measures the rain fall.</rdfs:label>
        <rdfs:label xml:lang="en">Pluviometer</rdfs:label>
    </owl:Class>
    


    <!-- https://w3id.org/def/saref4agri#SoilTensiometer -->

    <owl:Class rdf:about="https://w3id.org/def/saref4agri#SoilTensiometer">
        <rdfs:subClassOf rdf:resource="https://w3id.org/saref#Sensor"/>
        <rdfs:label xml:lang="en">A sensor that measures the soil moisture.</rdfs:label>
        <rdfs:label xml:lang="en">Soil tensiometer</rdfs:label>
    </owl:Class>
    


    <!-- https://w3id.org/def/saref4agri#WateringValve -->

    <owl:Class rdf:about="https://w3id.org/def/saref4agri#WateringValve">
        <rdfs:subClassOf rdf:resource="https://w3id.org/saref#Actuator"/>
        <rdfs:comment xml:lang="en">An actuator that open the water valve.</rdfs:comment>
        <rdfs:label xml:lang="en">WateringValve</rdfs:label>
    </owl:Class>
    


    <!-- https://w3id.org/def/saref4agri#WeatherStation -->

    <owl:Class rdf:about="https://w3id.org/def/saref4agri#WeatherStation">
        <rdfs:subClassOf rdf:resource="https://w3id.org/saref#Sensor"/>
        <rdfs:label xml:lang="en">A sensor o system that measure weather conditions.</rdfs:label>
        <rdfs:label xml:lang="en">Weather station</rdfs:label>
    </owl:Class>
    


    <!-- https://w3id.org/saref#Actuator -->

    <owl:Class rdf:about="https://w3id.org/saref#Actuator">
        <rdfs:subClassOf rdf:resource="https://w3id.org/saref#Device"/>
        <rdfs:isDefinedBy rdf:resource="https://w3id.org/saref#"/>
        <rdfs:label xml:lang="en">Actuator</rdfs:label>
    </owl:Class>
    


    <!-- https://w3id.org/saref#Command -->

    <owl:Class rdf:about="https://w3id.org/saref#Command">
        <rdfs:subClassOf>
            <owl:Restriction>
                <owl:onProperty rdf:resource="https://w3id.org/saref#isCommandOf"/>
                <owl:minQualifiedCardinality rdf:datatype="http://www.w3.org/2001/XMLSchema#nonNegativeInteger">1</owl:minQualifiedCardinality>
                <owl:onClass rdf:resource="https://w3id.org/saref#Function"/>
            </owl:Restriction>
        </rdfs:subClassOf>
        <rdfs:subClassOf>
            <owl:Restriction>
                <owl:onProperty rdf:resource="https://w3id.org/saref#hasDescription"/>
                <owl:maxCardinality rdf:datatype="http://www.w3.org/2001/XMLSchema#nonNegativeInteger">1</owl:maxCardinality>
            </owl:Restriction>
        </rdfs:subClassOf>
        <rdfs:comment>A directive that a device must support to perform a certain function. A command may act upon a state, but does not necessarily act upon a state. For example, the ON command acts upon the ON/OFF state, but the GET command does not act upon any state, it simply gives a directive to retrieve a certain value. We propose here a list of commands that are relevant for the purpose of SAREF, but this list can be extended.</rdfs:comment>
        <rdfs:label>Command</rdfs:label>
    </owl:Class>
    


    <!-- https://w3id.org/saref#Device -->

    <owl:Class rdf:about="https://w3id.org/saref#Device">
        <rdfs:subClassOf rdf:resource="http://www.w3.org/ns/ssn/System"/>
        <rdfs:isDefinedBy rdf:resource="https://w3id.org/saref#"/>
        <rdfs:label xml:lang="en">Device</rdfs:label>
    </owl:Class>
    


    <!-- https://w3id.org/saref#Function -->

    <owl:Class rdf:about="https://w3id.org/saref#Function">
        <rdfs:subClassOf>
            <owl:Restriction>
                <owl:onProperty rdf:resource="https://w3id.org/saref#hasCommand"/>
                <owl:minQualifiedCardinality rdf:datatype="http://www.w3.org/2001/XMLSchema#nonNegativeInteger">1</owl:minQualifiedCardinality>
                <owl:onClass rdf:resource="https://w3id.org/saref#Command"/>
            </owl:Restriction>
        </rdfs:subClassOf>
        <rdfs:comment xml:lang="en">The functionality necessary to accomplish the task for which a Device is designed. A device can be designed to perform more than one function. Functions can be structured in categories (subclasses) that reflect different points of view, for example, considering the specific application area for which a function can be used (e.g., light, temperature, motion, heat, power, etc.), or the capability that a function can support (e.g., receive, reply, notify, etc.), and so forth.</rdfs:comment>
        <rdfs:comment>The functionality necessary to accomplish the task for which a Device is designed. A device can be designed to perform more than one function. Functions can be structured in categories (subclasses) that reflect different points of view, for example, considering the specific application area for which a function can be used (e.g., light, temperature, motion, heat, power, etc.), or the capability that a function can support (e.g., receive, reply, notify, etc.), and so forth. </rdfs:comment>
        <rdfs:label>Function</rdfs:label>
        <rdfs:label xml:lang="en">Function</rdfs:label>
    </owl:Class>
    


    <!-- https://w3id.org/saref#Sensor -->

    <owl:Class rdf:about="https://w3id.org/saref#Sensor">
        <rdfs:subClassOf rdf:resource="https://w3id.org/saref#Device"/>
        <rdfs:isDefinedBy rdf:resource="https://w3id.org/saref#"/>
        <rdfs:label xml:lang="en">Sensor</rdfs:label>
    </owl:Class>
</rdf:RDF>



<!-- Generated by the OWL API (version 4.2.8.20170104-2310) https://github.com/owlcs/owlapi -->

